Split ChemicalDetector into several theories

examples/RoboChart/RoboChart_ChemicalDetector_autonomous/RoboChart_ChemicalDetector_autonomous.thy
@@ -3,984 +3,10 @@ text \<open> This theory aims for simulation of a trivial RoboChart model based 
  semantics. We use the @{term "rename"} operator for renaming.
 \<close>
 theory RoboChart_ChemicalDetector_autonomous
-  imports "../../ITree_RoboChart" "../../RC_Channel_Type" "../../Bounded_List" "../../Nat_Of"
+  imports "RoboChart_ChemicalDetector_autonomous_general"
 begin
 
 declare [[show_types]]
-
-subsection \<open> General definitions \<close>
-interpretation rc: robochart_confs "-2" "2" "2" "-2" "2".
-
-subsubsection \<open> Constants \<close>
-
-subsubsection \<open> Types \<close>
-
-(* PrimitiveType in RoboChart like given types in Z, and instantiated in CSP *)
-
-datatype ('a::finite) Chemical_Chem = Chemical_ChemC 'a
-
-abbreviation "Chemical_Chem2_list \<equiv> [Chemical_ChemC (0::2), Chemical_ChemC (1::2)]"
-abbreviation "Chemical_Chem2_set \<equiv> set Chemical_Chem2_list"
-
-definition Chemical_Chem_is_zero::"(2 Chemical_Chem) \<Rightarrow> bool" where
-"Chemical_Chem_is_zero x = (if x = (Chemical_ChemC (0::2)) then True else False)"
-
-value "Chemical_Chem_is_zero (Chemical_ChemC (3::2))"
-
-datatype ('a::finite) Chemical_Intensity = Chemical_IntensityC 'a
-
-abbreviation "Chemical_Intensity2_list \<equiv> [Chemical_IntensityC (0::2), Chemical_IntensityC 1]"
-abbreviation "Chemical_Intensity2_set \<equiv> set Chemical_Intensity2_list"
-
-definition Chemical_Intensity_is_zero::"(2 Chemical_Intensity) \<Rightarrow> bool" where
-"Chemical_Intensity_is_zero x = (if x = (Chemical_IntensityC (0::2)) then True else False)"
-
-fun Chemical_goreq :: "2 Chemical_Intensity \<Rightarrow> 2 Chemical_Intensity \<Rightarrow> bool" where
-"Chemical_goreq (Chemical_IntensityC x) (Chemical_IntensityC y) = (x \<ge> y) "
-
-text \<open> In CSP, LSeq(T,n) from core_defs.csp can be used as a type or an expression. In this 
-RoboChart model, it is used as a type, parametrised by n. We use bounded_list to implement it, 
-such as @{typ "int[2]blist"} for LSeq(int, 2).
-\<close>
-
-fun lseq where
-"lseq s 0 = [[]]" |
-"lseq s (Suc 0) = [[q]. q \<leftarrow> s]" |
-"lseq s (Suc n) = [q # qs. q \<leftarrow> s, qs \<leftarrow> (lseq s n)]"
-
-fun lseqn where
-"lseqn s 0 = lseq s 0" |
-"lseqn s (Suc n) = lseqn s n @ (lseq s (Suc n))"
-
-text \<open> Make a bounded list from the supplied list, a set of all possible elements. \<close>
-definition mk_blist :: "'n itself \<Rightarrow> 'a list \<Rightarrow> ('a['n::finite]blist) list" where
-"mk_blist _ xs = map (bmake TYPE('n)) (lseqn xs CARD('n))"
-
-subsection \<open> Chemical package \<close>
-enumtype Chemical_Status = 
-  Chemical_Status_noGas | Chemical_Status_gasD
-
-abbreviation "Chemical_Status_list \<equiv> enum_Chemical_Status_inst.enum_Chemical_Status"
-abbreviation "Chemical_Status_set \<equiv> set Chemical_Status_list"
-
-enumtype Chemical_Angle = 
-  Chemical_Angle_Left | Chemical_Angle_Right | 
-  Chemical_Angle_Back | Chemical_Angle_Front
-
-abbreviation "Chemical_Angle_list \<equiv> enum_Chemical_Angle_inst.enum_Chemical_Angle"
-abbreviation "Chemical_Angle_set \<equiv> set Chemical_Angle_list"
-
-text \<open> The angle function \<close>
-definition Chemical_angle :: "nat \<Rightarrow> Chemical_Angle" where
-"Chemical_angle x = (if x > 0 then Chemical_Angle_Right else Chemical_Angle_Front)"
-
-record 'a Chemical_GasSensor = 
-  c :: "'a Chemical_Chem"
-  i :: "'a Chemical_Intensity"
-
-type_synonym Chemical_GasSensor2 = "2 Chemical_GasSensor"
-
-definition Chemical_GasSensor2_list :: "Chemical_GasSensor2 list" where 
-"Chemical_GasSensor2_list \<equiv> 
-  [\<lparr>c = cc, i = ii\<rparr>. cc \<leftarrow> Chemical_Chem2_list, ii \<leftarrow> Chemical_Intensity2_list]"
-
-abbreviation "lseq_gassensor_enum \<equiv> mk_blist TYPE(2) Chemical_GasSensor2_list"
-
-(*
-function Chemical_analysis :: "2 Chemical_GasSensor[2]blist \<Rightarrow> Chemical_Status" where
-"Chemical_analysis (bmake TYPE(2) []) =  Chemical_Status_noGas" |
-"Chemical_analysis (bmake TYPE(2) (p#ps)) = 
-  (if Chemical_Chem_is_zero (c p) \<and> (Chemical_analysis (bmake TYPE(2) ps) = Chemical_Status_noGas) 
-   then Chemical_Status_noGas else Chemical_Status_gasD)"
-     apply (auto)
-*)
-
-function Chemical_analysis :: "2 Chemical_GasSensor[2]blist \<Rightarrow> Chemical_Status" where
-"Chemical_analysis (gs) = 
-  (case list_of_blist gs of
-    []      \<Rightarrow> Chemical_Status_noGas |
-    (p#ps)  \<Rightarrow> (if Chemical_Chem_is_zero (c p) \<and> 
-                  (Chemical_analysis (bmake TYPE(2) ps) = Chemical_Status_noGas) 
-                then Chemical_Status_noGas
-                else Chemical_Status_gasD)
-  )"
-  by auto
-
-termination Chemical_analysis 
-  apply (relation "measure (\<lambda> gs. blength gs)")
-  apply (auto)
-proof -
-  fix gs::"2 Chemical_GasSensor [2]blist" and 
-      x21::"2 Chemical_GasSensor" and 
-      x22::"2 Chemical_GasSensor list"
-  assume a1: "list_of_blist gs = x21 # x22"
-  from a1 have f1: "blength gs > 0"
-    by (simp add: blength_def)
-  show "blength (bmake TYPE(2) x22) < blength gs"
-    by (metis a1 blist_remove_head f1 list.sel(3))
-qed
-
-value "Chemical_analysis (bmake TYPE(2) [])"
-value "Chemical_analysis (bmake TYPE(2) [\<lparr>c = Chemical_ChemC (0::2), i = Chemical_IntensityC (0::2)\<rparr>])"
-
-text \<open> The intensity function \<close>
-definition pre_Chemical_intensity :: "2 Chemical_GasSensor[2]blist \<Rightarrow> bool" where
-"pre_Chemical_intensity gs = (blength gs > 0)"
-
-function Chemical_intensity :: "2 Chemical_GasSensor[2]blist \<Rightarrow> (2 Chemical_Intensity)" where
-"Chemical_intensity (gs) = 
-  (case list_of_blist gs of
-    []      \<Rightarrow> Chemical_IntensityC (0::2) |
-    (p#ps)  \<Rightarrow> (if Chemical_goreq (i p) (Chemical_intensity (bmake TYPE(2) ps)) 
-                then i p
-                else Chemical_intensity (bmake TYPE(2) ps))
-  )"
-  by auto
-
-termination Chemical_intensity 
-  apply (relation "measure (\<lambda> gs. blength gs)")
-  apply (auto)
-  by (metis add_Suc_right blength.rep_eq blist_remove_head less_nat_zero_code linorder_cases 
-      list.sel(3) list.size(4) nat.simps(3))+
-
-value "Chemical_intensity (bmake TYPE(2) [])"
-value "Chemical_intensity (bmake TYPE(2) 
-  [\<lparr>c = Chemical_ChemC (0::2), i = Chemical_IntensityC (1::2)\<rparr>,
-   \<lparr>c = Chemical_ChemC (1::2), i = Chemical_IntensityC (0::2)\<rparr>])"
-
-text \<open> The location function \<close>
-definition pre_Chemical_location :: "2 Chemical_GasSensor[2]blist \<Rightarrow> bool" where
-"pre_Chemical_location gs = (blength gs > 0)"
-
-function Chemical_location' :: "2 Chemical_GasSensor[2]blist \<Rightarrow> nat \<Rightarrow> (Chemical_Angle)" where
-"Chemical_location' (gs) x = 
-  (case list_of_blist gs of
-    []      \<Rightarrow> Chemical_angle(x) |
-    (p#ps)  \<Rightarrow> (if (i p) = (Chemical_intensity (gs))
-                then Chemical_angle(x)
-                else Chemical_location' (bmake TYPE(2) ps) (x+1)
-               )
-  )"
-  by auto
-
-termination Chemical_location'
-  apply (relation "measure (\<lambda> (gs, n). blength gs)")
-  apply (auto)
-  by (metis add_Suc_right blength.rep_eq blist_remove_head less_nat_zero_code linorder_cases 
-      list.sel(3) list.size(4) nat.simps(3))+
-
-abbreviation "Chemical_location gs \<equiv> Chemical_location' gs 0"
-
-value "Chemical_location (bmake TYPE(2) [])"
-value "Chemical_location (bmake TYPE(2) 
-  [\<lparr>c = Chemical_ChemC (0::2), i = Chemical_IntensityC (0::2)\<rparr>,
-   \<lparr>c = Chemical_ChemC (1::2), i = Chemical_IntensityC (1::2)\<rparr>])"
-
-subsection \<open> Location package \<close>
-enumtype Location_Loc = 
-  Location_Loc_left | Location_Loc_right | Location_Loc_front
-
-subsection \<open> GasAnalysis \<close>
-definition "const_GasAnalysis_thr \<equiv> Chemical_IntensityC (1::2)"
-
-enumtype SIDS_GasAnalysis = SID_GasAnalysis
-	              | SID_GasAnalysis_NoGas
-	              | SID_GasAnalysis_Analysis
-	              | SID_GasAnalysis_GasDetected
-	              | SID_GasAnalysis_j1
-	              | SID_GasAnalysis_Reading
-
-definition "SIDS_GasAnalysis_list = enum_SIDS_GasAnalysis_inst.enum_SIDS_GasAnalysis"
-definition "SIDS_GasAnalysis_set = set SIDS_GasAnalysis_list"
-definition "SIDS_GasAnalysis_nodes = (removeAll SID_GasAnalysis SIDS_GasAnalysis_list)"
-definition "SIDS_GasAnalysis_no_NoGas = (removeAll SID_GasAnalysis_NoGas SIDS_GasAnalysis_list)"
-definition "SIDS_GasAnalysis_no_Analysis = (removeAll SID_GasAnalysis_Analysis SIDS_GasAnalysis_list)"
-definition "SIDS_GasAnalysis_no_GasDetected = (removeAll SID_GasAnalysis_GasDetected SIDS_GasAnalysis_list)"
-definition "SIDS_GasAnalysis_no_Reading = (removeAll SID_GasAnalysis_Reading SIDS_GasAnalysis_list)"
-definition "SIDS_GasAnalysis_no_j1 = (removeAll SID_GasAnalysis_j1 SIDS_GasAnalysis_list)"
-
-enumtype TIDS_GasAnalysis = NULLTRANSITION__GasAnalysis
-	              | TID_GasAnalysis_t1
-	              | TID_GasAnalysis_t2
-	              | TID_GasAnalysis_t3
-	              | TID_GasAnalysis_t4
-	              | TID_GasAnalysis_t8
-	              | TID_GasAnalysis_t9a
-	              | TID_GasAnalysis_t0
-
-definition "TIDS_GasAnalysis_list = enum_TIDS_GasAnalysis_inst.enum_TIDS_GasAnalysis"
-definition "TIDS_GasAnalysis_set = set TIDS_GasAnalysis_list"
-
-text \<open> Identifiers of transitions that can interrupt a state, excluding transitions from junctions. \<close>
-definition "ITIDS_GasAnalysis_list = [TID_GasAnalysis_t0, 
-  TID_GasAnalysis_t2, TID_GasAnalysis_t3,	TID_GasAnalysis_t4,	
-  TID_GasAnalysis_t8,	TID_GasAnalysis_t9a
-]"
-
-definition "ITIDS_GasAnalysis = set ITIDS_GasAnalysis_list"
-
-chantype Chan_GasAnalysis =
-(* flow channels *)
-  internal_GasAnalysis :: TIDS_GasAnalysis
-  enter_GasAnalysis :: "SIDS_GasAnalysis \<times> SIDS_GasAnalysis"
-  entered_GasAnalysis :: "SIDS_GasAnalysis \<times> SIDS_GasAnalysis"
-  exit_GasAnalysis :: "SIDS_GasAnalysis \<times> SIDS_GasAnalysis"
-  exited_GasAnalysis :: "SIDS_GasAnalysis \<times> SIDS_GasAnalysis"
-  terminate_GasAnalysis :: unit
-
-(* Variables *)
-  get_st_GasAnalysis :: Chemical_Status
-  set_st_GasAnalysis :: Chemical_Status
-  get_gs_GasAnalysis :: "2 Chemical_GasSensor[2]blist" (* "Chemical_GasSensor LSeq"*)
-  set_gs_GasAnalysis :: "2 Chemical_GasSensor[2]blist"
-  get_i_GasAnalysis :: "2 Chemical_Intensity"
-  set_i_GasAnalysis :: "2 Chemical_Intensity"
-  get_a_GasAnalysis :: "Chemical_Angle"
-  set_a_GasAnalysis :: "Chemical_Angle"
-
-(* event channels *)
-  gas__GasAnalysis :: "TIDS_GasAnalysis \<times> InOut \<times> 2 Chemical_GasSensor[2]blist"
-  gas_GasAnalysis :: "InOut \<times> 2 Chemical_GasSensor[2]blist"
-  resume__GasAnalysis :: "TIDS_GasAnalysis \<times> InOut"
-  resume_GasAnalysis :: "InOut"
-  turn__GasAnalysis :: "TIDS_GasAnalysis \<times> InOut \<times> Chemical_Angle"
-  turn_GasAnalysis :: "InOut \<times> Chemical_Angle"
-  stop__GasAnalysis :: "TIDS_GasAnalysis \<times> InOut"
-  stop_GasAnalysis :: "InOut"
-
-subsubsection \<open> Sets of events \<close>
-(* How to use a list to represent all possible values of Chemical_GasSensor[2]blist *)
-definition int_int_GasAnalysis where
-"int_int_GasAnalysis = set (
-  (enumchans3 [gas__GasAnalysis_C] 
-    [TID_GasAnalysis_t0, TID_GasAnalysis_t2, 
-     TID_GasAnalysis_t3, TID_GasAnalysis_t4,
-     TID_GasAnalysis_t8, TID_GasAnalysis_t9a] 
-    [din, dout] 
-    (lseq_gassensor_enum)) @
-  (enumchans2 [resume__GasAnalysis_C] 
-    [TID_GasAnalysis_t0, TID_GasAnalysis_t2, 
-     TID_GasAnalysis_t3, TID_GasAnalysis_t4,
-     TID_GasAnalysis_t8, TID_GasAnalysis_t9a] 
-    [din, dout]) @
-  (enumchans3 [turn__GasAnalysis_C] 
-    [TID_GasAnalysis_t0, TID_GasAnalysis_t2, 
-     TID_GasAnalysis_t3, TID_GasAnalysis_t4,
-     TID_GasAnalysis_t8, TID_GasAnalysis_t9a] 
-    [din, dout]
-    Chemical_Angle_list
-    ) @
-  (enumchans2 [stop__GasAnalysis_C] 
-    [TID_GasAnalysis_t0, TID_GasAnalysis_t2, 
-     TID_GasAnalysis_t3, TID_GasAnalysis_t4,
-     TID_GasAnalysis_t8, TID_GasAnalysis_t9a] 
-    [din, dout]  
-    ) @
-  (enumchan1 internal_GasAnalysis_C 
-    [TID_GasAnalysis_t0, TID_GasAnalysis_t2, 
-     TID_GasAnalysis_t3, TID_GasAnalysis_t4,
-     TID_GasAnalysis_t8, TID_GasAnalysis_t9a])
-)"
-
-abbreviation "enter_exit_channels_GasAnalysis \<equiv>
-  [enter_GasAnalysis_C, entered_GasAnalysis_C, exit_GasAnalysis_C, exited_GasAnalysis_C]"
-
-definition internal_events_GasAnalysis where
-"internal_events_GasAnalysis = set (
-  enumchans2 enter_exit_channels_GasAnalysis SIDS_GasAnalysis_list SIDS_GasAnalysis_list
-)"
-
-
-definition GasAnalysis_i_events where
-"GasAnalysis_i_events = 
-    set (enumchans1 [get_i_GasAnalysis_C, set_i_GasAnalysis_C] Chemical_Intensity2_list)
-"
-
-definition GasAnalysis_st_events where
-"GasAnalysis_st_events = 
-    set (enumchans1 [get_st_GasAnalysis_C, set_st_GasAnalysis_C] Chemical_Status_list)
-"
-
-definition GasAnalysis_gs_events where
-"GasAnalysis_gs_events = 
-    set (enumchans1 [get_gs_GasAnalysis_C, set_gs_GasAnalysis_C] lseq_gassensor_enum)
-"
-
-definition GasAnalysis_a_events where
-"GasAnalysis_a_events = 
-    set (enumchans1 [get_a_GasAnalysis_C, set_a_GasAnalysis_C] Chemical_Angle_list)
-"
-
-definition GasAnalysis_MachineInternalEvents where
-"GasAnalysis_MachineInternalEvents = 
-  set (enumchan1 internal_GasAnalysis_C TIDS_GasAnalysis_list)
-"
-
-subsubsection \<open> State Machine Memory \<close>
-text \<open> Memory cell processes \<close>
-
-(* for the local variable x *)
-definition GasAnalysis_Memory_opt_gs where
-"GasAnalysis_Memory_opt_gs = 
-  mem_of_lvar get_gs_GasAnalysis set_gs_GasAnalysis 
-    (set (lseq_gassensor_enum))"
-
-definition GasAnalysis_Memory_opt_a where
-"GasAnalysis_Memory_opt_a = mem_of_lvar get_a_GasAnalysis set_a_GasAnalysis Chemical_Angle_set"
-
-definition GasAnalysis_Memory_opt_i where
-"GasAnalysis_Memory_opt_i = mem_of_lvar get_i_GasAnalysis set_i_GasAnalysis (Chemical_Intensity2_set)"
-
-definition GasAnalysis_Memory_opt_st where
-"GasAnalysis_Memory_opt_st = mem_of_lvar get_st_GasAnalysis set_st_GasAnalysis (Chemical_Status_set)"
-
-text \<open> Memory transition processes \<close>
-definition GasAnalysis_MemoryTransitions_opt_0 where
-"GasAnalysis_MemoryTransitions_opt_0 = 
-  loop (\<lambda> id::integer. 
-    (do {outp internal_GasAnalysis TID_GasAnalysis_t1 ; Ret (id)} \<box> 
-     do {gs \<leftarrow> inp_in gas__GasAnalysis (set [(TID_GasAnalysis_t2, din, x). 
-              x \<leftarrow> (lseq_gassensor_enum)]) ; Ret (id)}  \<box> 
-     do {gs \<leftarrow> inp_in gas__GasAnalysis (set [(TID_GasAnalysis_t0, din, x). 
-              x \<leftarrow> (lseq_gassensor_enum)]) ; Ret (id)})
-  )
-"
-
-definition GasAnalysis_MemoryTransitions_opt_1 where
-"GasAnalysis_MemoryTransitions_opt_1 = 
-  loop (\<lambda> id::integer.
-    do {st \<leftarrow> inp_in get_st_GasAnalysis Chemical_Status_set ; 
-      (
-        do {guard (st = Chemical_Status_gasD); outp internal_GasAnalysis TID_GasAnalysis_t4 ; Ret (id)} \<box>
-        do {guard (st = Chemical_Status_noGas); outp internal_GasAnalysis TID_GasAnalysis_t3 ; Ret (id)} \<box>
-        do {x \<leftarrow> inp_in set_st_GasAnalysis Chemical_Status_set; Ret (id)}
-      )
-    }
-  )
-"
-
-definition GasAnalysis_MemoryTransitions_opt_2 where
-"GasAnalysis_MemoryTransitions_opt_2 = 
-  loop (\<lambda> id::integer.
-    do {i \<leftarrow> inp_in get_i_GasAnalysis Chemical_Intensity2_set ; 
-      (
-        do {guard (\<not> (Chemical_goreq i const_GasAnalysis_thr)); outp internal_GasAnalysis TID_GasAnalysis_t9a ; Ret (id)} \<box>
-        do {guard (Chemical_goreq i const_GasAnalysis_thr); outp internal_GasAnalysis TID_GasAnalysis_t8 ; Ret (id)} \<box>
-        do {x \<leftarrow> inp_in set_i_GasAnalysis Chemical_Intensity2_set; Ret (id)}
-      )
-    }
-  )
-"
-
-subsubsection \<open> States \<close>
-paragraph \<open> Initial \<close>
-definition I_GasAnalysis_i1 where
-"I_GasAnalysis_i1 = (\<lambda> (id::integer) . 
-  do {outp internal_GasAnalysis TID_GasAnalysis_t1 ; 
-      outp enter_GasAnalysis (SID_GasAnalysis, SID_GasAnalysis_NoGas);
-      outp entered_GasAnalysis (SID_GasAnalysis, SID_GasAnalysis_NoGas)
-  })
-"
-
-paragraph \<open> NoGas \<close>
-definition CS_GasAnalysis_NoGas_sync where
-"CS_GasAnalysis_NoGas_sync = 
-  set (
-      \<comment> \<open> enter from x to y \<close>
-      (enumchans2 enter_exit_channels_GasAnalysis [SID_GasAnalysis_NoGas] SIDS_GasAnalysis_nodes)@
-      \<comment> \<open> enter from y to x \<close>
-      (enumchans2 enter_exit_channels_GasAnalysis SIDS_GasAnalysis_nodes [SID_GasAnalysis_NoGas])
-)"
-
-definition GasAnalysis_NoGas_triggers where
-"GasAnalysis_NoGas_triggers = set (
-  (enumchan1 internal_GasAnalysis_C 
-    [TID_GasAnalysis_t3, TID_GasAnalysis_t4,
-     TID_GasAnalysis_t8, TID_GasAnalysis_t9a]) @
-  (enumchans3 [gas__GasAnalysis_C] 
-    [TID_GasAnalysis_t0, TID_GasAnalysis_t2] 
-    [din, dout] 
-    (lseq_gassensor_enum))
-)
-"
-
-definition tids_GasAnalysis_NoGas where
-" tids_GasAnalysis_NoGas = 
-    (filter 
-        (\<lambda> s. s \<notin> {NULLTRANSITION__GasAnalysis, TID_GasAnalysis_t9a,
-          TID_GasAnalysis_t8, TID_GasAnalysis_t4, TID_GasAnalysis_t3, 
-          TID_GasAnalysis_t2, TID_GasAnalysis_t0}) 
-        ITIDS_GasAnalysis_list)"
-
-abbreviation Other_SIDs_to_NoGas_GasAnalysis where
-"Other_SIDs_to_NoGas_GasAnalysis \<equiv>
-  set [(s, SID_GasAnalysis_NoGas) . s \<leftarrow> (SIDS_GasAnalysis_no_NoGas)]"
-
-definition 
-"exit_events_GasAnalysis idd sid tids other_sids =
-    (do {inp_in internal_GasAnalysis (set tids);
-        y \<leftarrow> inp_in exit_GasAnalysis other_sids;
-          outp exited_GasAnalysis (fst y, sid);
-          Ret(False, idd, sid)
-        } \<box>
-    do {t \<leftarrow> inp_in gas__GasAnalysis (set [(t, d, gs). 
-            t \<leftarrow> (tids), d \<leftarrow> InOut_list,
-            gs \<leftarrow> (lseq_gassensor_enum)]) ;
-          y \<leftarrow> inp_in exit_GasAnalysis other_sids;
-            outp exited_GasAnalysis (fst y, sid);
-            Ret(False, idd, sid)
-        } \<box>
-    do {t \<leftarrow> inp_in resume__GasAnalysis (set [(t, d). 
-            t \<leftarrow> (tids), d \<leftarrow> InOut_list]) ;
-          y \<leftarrow> inp_in exit_GasAnalysis other_sids;
-            outp exited_GasAnalysis (fst y, sid);
-            Ret(False, idd, sid)
-        } \<box>
-    do {t \<leftarrow> inp_in turn__GasAnalysis (set [(t, d, a). 
-            t \<leftarrow> (tids), d \<leftarrow> InOut_list,
-            a \<leftarrow> Chemical_Angle_list]) ;
-          y \<leftarrow> inp_in exit_GasAnalysis other_sids;
-            outp exited_GasAnalysis (fst y, sid);
-            Ret(False, idd, sid)
-        } \<box>
-    do {t \<leftarrow> inp_in stop__GasAnalysis (set [(t, d). 
-            t \<leftarrow> (tids), d \<leftarrow> InOut_list]) ;
-          y \<leftarrow> inp_in exit_GasAnalysis other_sids;
-            outp exited_GasAnalysis (fst y, sid);
-            Ret(False, idd, sid)
-        }
-    )"
-
-definition State_GasAnalysis_NoGas where 
-"State_GasAnalysis_NoGas = 
-  loop (\<lambda> (id::integer).
-    do {sd \<leftarrow> inp_in enter_GasAnalysis Other_SIDs_to_NoGas_GasAnalysis ; 
-        \<comment> \<open> State passed to next loop, including a condition initially True. \<close>
-        ret \<leftarrow> Ret (True, id, fst sd) ; 
-        \<comment> \<open> State_GasAnalysis_NoGas_execute \<close>
-        (iterate 
-           \<comment> \<open> condition \<close>
-           (\<lambda> s. fst s) 
-           \<comment> \<open> P \<close>
-           (\<lambda> s.
-            do {
-              outp entered_GasAnalysis (snd (snd s), SID_GasAnalysis_NoGas);
-              (do {skip ; stop} \<triangle>
-                (
-                \<comment> \<open> T_GasAnalysis_t2 \<close>
-                do {t \<leftarrow> inp_in gas__GasAnalysis (set [(TID_GasAnalysis_t2, din, gs). 
-                                gs \<leftarrow> (lseq_gassensor_enum)]) ;
-                      outp set_gs_GasAnalysis (snd (snd t)) ; 
-                      outp exit_GasAnalysis (SID_GasAnalysis_NoGas, SID_GasAnalysis_NoGas);
-                      outp exited_GasAnalysis (SID_GasAnalysis_NoGas, SID_GasAnalysis_NoGas);
-                      outp enter_GasAnalysis (SID_GasAnalysis_NoGas, SID_GasAnalysis_Analysis);
-                      outp entered_GasAnalysis (SID_GasAnalysis_NoGas, SID_GasAnalysis_Analysis);
-                      Ret(False, fst (snd s), SID_GasAnalysis_NoGas)
-                    } \<box>
-                (exit_events_GasAnalysis (fst (snd s)) SID_GasAnalysis_NoGas 
-                   tids_GasAnalysis_NoGas Other_SIDs_to_NoGas_GasAnalysis)
-                )
-              )
-            })
-            \<comment> \<open> The previous state: a triple \<close> 
-            (ret)
-        ) ;
-        Ret (id)
-  }
-)
-"
-
-definition State_GasAnalysis_NoGas_R where
-"State_GasAnalysis_NoGas_R (idd::integer) = 
-   (discard_state (State_GasAnalysis_NoGas idd)) \<comment> \<open> discard state to match with skip on the right\<close>
-    \<parallel>\<^bsub> (int_int_GasAnalysis - GasAnalysis_NoGas_triggers) \<^esub> 
-   skip
-"
-
-paragraph \<open> Analysis \<close>
-definition CS_GasAnalysis_Analysis_sync where
-"CS_GasAnalysis_Analysis_sync = 
-  set (
-      \<comment> \<open> enter from x to y \<close>
-      (enumchans2 enter_exit_channels_GasAnalysis [SID_GasAnalysis_Analysis] SIDS_GasAnalysis_nodes)@
-      \<comment> \<open> enter from y to x \<close>
-      (enumchans2 enter_exit_channels_GasAnalysis SIDS_GasAnalysis_nodes [SID_GasAnalysis_Analysis])
-)"
-
-definition GasAnalysis_Analysis_triggers where
-"GasAnalysis_Analysis_triggers = set (
-  (enumchan1 internal_GasAnalysis_C 
-    [TID_GasAnalysis_t3, TID_GasAnalysis_t4,
-     TID_GasAnalysis_t8, TID_GasAnalysis_t9a]) @
-  (enumchans3 [gas__GasAnalysis_C] 
-    [TID_GasAnalysis_t0, TID_GasAnalysis_t2] 
-    [din, dout] 
-    (lseq_gassensor_enum))
-)
-"
-
-definition tids_GasAnalysis_Analysis where
-" tids_GasAnalysis_Analysis = 
-    (filter 
-        (\<lambda> s. s \<notin> {NULLTRANSITION__GasAnalysis, TID_GasAnalysis_t9a,
-          TID_GasAnalysis_t8, TID_GasAnalysis_t4, TID_GasAnalysis_t3, 
-          TID_GasAnalysis_t2, TID_GasAnalysis_t0}) 
-        ITIDS_GasAnalysis_list)"
-
-abbreviation Other_SIDs_to_Analysis_GasAnalysis where
-"Other_SIDs_to_Analysis_GasAnalysis \<equiv> 
-  set [(s, SID_GasAnalysis_Analysis) . s \<leftarrow> (SIDS_GasAnalysis_no_Analysis)]"
-
-definition State_GasAnalysis_Analysis where 
-"State_GasAnalysis_Analysis = 
-  loop (\<lambda> (id::integer).
-    do {sd \<leftarrow> inp_in enter_GasAnalysis Other_SIDs_to_Analysis_GasAnalysis ; 
-        \<comment> \<open> State passed to next loop, including a condition initially True. \<close>
-        ret \<leftarrow> Ret (True, id, fst sd) ; 
-        \<comment> \<open> State_GasAnalysis_Analysis_execute \<close>
-        (iterate 
-           \<comment> \<open> condition \<close>
-           (\<lambda> s. fst s) 
-           \<comment> \<open> P \<close>
-           (\<lambda> s.
-            do {
-              gs \<leftarrow> inp_in get_gs_GasAnalysis (set (lseq_gassensor_enum));
-              outp set_st_GasAnalysis (Chemical_analysis gs);
-              outp entered_GasAnalysis (snd (snd s), SID_GasAnalysis_Analysis);
-              (do {skip ; stop} \<triangle>
-                (
-                \<comment> \<open> T_GasAnalysis_t3 \<close>
-                do {outp internal_GasAnalysis TID_GasAnalysis_t3 ;
-                    outp exit_GasAnalysis (SID_GasAnalysis_Analysis, SID_GasAnalysis_Analysis);
-                    outp exited_GasAnalysis (SID_GasAnalysis_Analysis, SID_GasAnalysis_Analysis);
-                    outp resume_GasAnalysis dout;
-                    outp enter_GasAnalysis (SID_GasAnalysis_Analysis, SID_GasAnalysis_NoGas);
-                    outp entered_GasAnalysis (SID_GasAnalysis_Analysis, SID_GasAnalysis_NoGas);
-                    Ret(False, fst (snd s), SID_GasAnalysis_Analysis)
-                    } \<box>
-                \<comment> \<open> T_GasAnalysis_t4 \<close>
-                do {outp internal_GasAnalysis TID_GasAnalysis_t4 ;
-                    outp exit_GasAnalysis (SID_GasAnalysis_Analysis, SID_GasAnalysis_Analysis);
-                    outp exited_GasAnalysis (SID_GasAnalysis_Analysis, SID_GasAnalysis_Analysis);
-                    outp enter_GasAnalysis (SID_GasAnalysis_Analysis, SID_GasAnalysis_GasDetected);
-                    outp entered_GasAnalysis (SID_GasAnalysis_Analysis, SID_GasAnalysis_GasDetected);
-                    Ret(False, fst (snd s), SID_GasAnalysis_Analysis)
-                    } \<box>
-                (exit_events_GasAnalysis (fst (snd s)) SID_GasAnalysis_Analysis 
-                   tids_GasAnalysis_Analysis Other_SIDs_to_Analysis_GasAnalysis)
-                )
-              )
-            })
-            \<comment> \<open> The previous state: a triple \<close> 
-            (ret)
-        ) ;
-        Ret (id)
-  }
-)
-"
-
-definition State_GasAnalysis_Analysis_R where
-"State_GasAnalysis_Analysis_R (idd::integer) = 
-   (discard_state (State_GasAnalysis_Analysis idd)) \<comment> \<open> discard state to match with skip on the right\<close>
-    \<parallel>\<^bsub> (int_int_GasAnalysis - GasAnalysis_Analysis_triggers) \<^esub> 
-   skip
-"
-
-paragraph \<open> GasDetected \<close>
-definition CS_GasAnalysis_GasDetected_sync where
-"CS_GasAnalysis_GasDetected_sync = 
-  set (
-      \<comment> \<open> enter from x to y \<close>
-      (enumchans2 enter_exit_channels_GasAnalysis [SID_GasAnalysis_GasDetected] SIDS_GasAnalysis_nodes)@
-      \<comment> \<open> enter from y to x \<close>
-      (enumchans2 enter_exit_channels_GasAnalysis SIDS_GasAnalysis_nodes [SID_GasAnalysis_GasDetected])
-)"
-
-definition GasAnalysis_GasDetected_triggers where
-"GasAnalysis_GasDetected_triggers = set (
-  (enumchan1 internal_GasAnalysis_C 
-    [TID_GasAnalysis_t3, TID_GasAnalysis_t4,
-     TID_GasAnalysis_t8, TID_GasAnalysis_t9a]) @
-  (enumchans3 [gas__GasAnalysis_C] 
-    [TID_GasAnalysis_t0, TID_GasAnalysis_t2] 
-    [din, dout] 
-    (lseq_gassensor_enum))
-)
-"
-
-definition tids_GasAnalysis_GasDetected where
-" tids_GasAnalysis_GasDetected = 
-    (filter 
-        (\<lambda> s. s \<notin> {NULLTRANSITION__GasAnalysis, TID_GasAnalysis_t9a,
-          TID_GasAnalysis_t8, TID_GasAnalysis_t4, TID_GasAnalysis_t3, 
-          TID_GasAnalysis_t2, TID_GasAnalysis_t0}) 
-        ITIDS_GasAnalysis_list)"
-
-abbreviation Other_SIDs_to_GasDetected_GasAnalysis where
-"Other_SIDs_to_GasDetected_GasAnalysis \<equiv>
-  set [(s, SID_GasAnalysis_GasDetected) . s \<leftarrow> (SIDS_GasAnalysis_no_GasDetected)]"
-
-definition State_GasAnalysis_GasDetected where 
-"State_GasAnalysis_GasDetected = 
-  loop (\<lambda> (id::integer).
-    do {sd \<leftarrow> inp_in enter_GasAnalysis Other_SIDs_to_GasDetected_GasAnalysis ; 
-        \<comment> \<open> State passed to next loop, including a condition initially True. \<close>
-        ret \<leftarrow> Ret (True, id, fst sd) ; 
-        \<comment> \<open> State_GasAnalysis_GasDetected_execute \<close>
-        (iterate 
-           \<comment> \<open> condition \<close>
-           (\<lambda> s. fst s) 
-           \<comment> \<open> P \<close>
-           (\<lambda> s.
-            do {
-              gs \<leftarrow> inp_in get_gs_GasAnalysis (set (lseq_gassensor_enum));
-              guard (pre_Chemical_intensity(gs));
-              outp set_i_GasAnalysis (Chemical_intensity gs);
-              outp entered_GasAnalysis (snd (snd s), SID_GasAnalysis_GasDetected);
-              (do {skip ; stop} \<triangle>
-                (
-                \<comment> \<open> T_GasAnalysis_t8 \<close>
-                do {outp internal_GasAnalysis TID_GasAnalysis_t8 ;
-                    outp exit_GasAnalysis (SID_GasAnalysis_GasDetected, SID_GasAnalysis_GasDetected);
-                    outp exited_GasAnalysis (SID_GasAnalysis_GasDetected, SID_GasAnalysis_GasDetected);
-                    outp stop_GasAnalysis dout;
-                    outp enter_GasAnalysis (SID_GasAnalysis_GasDetected, SID_GasAnalysis_j1);
-                    outp entered_GasAnalysis (SID_GasAnalysis_GasDetected, SID_GasAnalysis_j1);
-                    Ret(False, fst (snd s), SID_GasAnalysis_GasDetected)
-                    } \<box>
-                 \<comment> \<open> T_GasAnalysis_t9a \<close>
-                do {outp internal_GasAnalysis TID_GasAnalysis_t9a ;
-                    outp exit_GasAnalysis (SID_GasAnalysis_GasDetected, SID_GasAnalysis_GasDetected);
-                    outp exited_GasAnalysis (SID_GasAnalysis_GasDetected, SID_GasAnalysis_GasDetected);
-                    gs \<leftarrow> inp_in get_gs_GasAnalysis (set (lseq_gassensor_enum));
-                    guard (pre_Chemical_location(gs));
-                    outp set_a_GasAnalysis (Chemical_location gs);
-                    a \<leftarrow> inp_in get_a_GasAnalysis Chemical_Angle_set;
-                    outp turn_GasAnalysis (dout, a);
-                    outp enter_GasAnalysis (SID_GasAnalysis_GasDetected, SID_GasAnalysis_Reading);
-                    outp entered_GasAnalysis (SID_GasAnalysis_GasDetected, SID_GasAnalysis_Reading);
-                    Ret(False, fst (snd s), SID_GasAnalysis_GasDetected)
-                    } \<box>
-                (exit_events_GasAnalysis (fst (snd s)) SID_GasAnalysis_GasDetected 
-                   tids_GasAnalysis_GasDetected Other_SIDs_to_GasDetected_GasAnalysis)
-                )
-              )
-            })
-            \<comment> \<open> The previous state: a triple \<close> 
-            (ret)
-        ) ;
-        Ret (id)
-  }
-)
-"
-
-definition State_GasAnalysis_GasDetected_R where
-"State_GasAnalysis_GasDetected_R (idd::integer) = 
-   (discard_state (State_GasAnalysis_GasDetected idd)) \<comment> \<open> discard state to match with skip on the right\<close>
-    \<parallel>\<^bsub> (int_int_GasAnalysis - GasAnalysis_GasDetected_triggers) \<^esub> 
-   skip
-"
-
-paragraph \<open> Final \<close>
-definition CS_GasAnalysis_j1_sync where
-"CS_GasAnalysis_j1_sync = 
-  set (
-      \<comment> \<open> enter from x to y \<close>
-      (enumchans2 enter_exit_channels_GasAnalysis [SID_GasAnalysis_j1] SIDS_GasAnalysis_nodes)@
-      \<comment> \<open> enter from y to x \<close>
-      (enumchans2 enter_exit_channels_GasAnalysis SIDS_GasAnalysis_nodes [SID_GasAnalysis_j1])
-)"
-
-definition GasAnalysis_j1_triggers where
-"GasAnalysis_j1_triggers = set ([])
-"
-
-definition tids_GasAnalysis_j1 where
-" tids_GasAnalysis_j1 = 
-    (filter 
-        (\<lambda> s. s \<notin> {NULLTRANSITION__GasAnalysis, TID_GasAnalysis_t9a,
-          TID_GasAnalysis_t8, TID_GasAnalysis_t4, TID_GasAnalysis_t3, 
-          TID_GasAnalysis_t2, TID_GasAnalysis_t0}) 
-        ITIDS_GasAnalysis_list)"
-
-abbreviation Other_SIDs_to_j1_GasAnalysis where
-"Other_SIDs_to_j1_GasAnalysis \<equiv>
-  set [(s, SID_GasAnalysis_j1) . s \<leftarrow> (SIDS_GasAnalysis_no_j1)]"
-
-definition State_GasAnalysis_j1 where 
-"State_GasAnalysis_j1 = 
-  loop (\<lambda> (id::integer).
-    do {sd \<leftarrow> inp_in enter_GasAnalysis Other_SIDs_to_j1_GasAnalysis ; 
-        outp terminate_GasAnalysis ();
-        Ret (id)
-    }
-)
-"
-
-definition State_GasAnalysis_j1_R where
-"State_GasAnalysis_j1_R (idd::integer) = 
-   (discard_state (State_GasAnalysis_j1 idd)) \<comment> \<open> discard state to match with skip on the right\<close>
-    \<parallel>\<^bsub> (int_int_GasAnalysis - GasAnalysis_j1_triggers) \<^esub> 
-   skip
-"
-
-paragraph \<open> Reading \<close>
-definition CS_GasAnalysis_Reading_sync where
-"CS_GasAnalysis_Reading_sync = 
-  set (
-      \<comment> \<open> enter from x to y \<close>
-      (enumchans2 enter_exit_channels_GasAnalysis [SID_GasAnalysis_Reading] SIDS_GasAnalysis_nodes)@
-      \<comment> \<open> enter from y to x \<close>
-      (enumchans2 enter_exit_channels_GasAnalysis SIDS_GasAnalysis_nodes [SID_GasAnalysis_Reading])
-)"
-
-definition GasAnalysis_Reading_triggers where
-"GasAnalysis_Reading_triggers = set (
-  (enumchan1 internal_GasAnalysis_C 
-    [TID_GasAnalysis_t3, TID_GasAnalysis_t4,
-     TID_GasAnalysis_t8, TID_GasAnalysis_t9a]) @
-  (enumchans3 [gas__GasAnalysis_C] 
-    [TID_GasAnalysis_t0, TID_GasAnalysis_t2] 
-    [din, dout] 
-    (lseq_gassensor_enum))
-)
-"
-
-definition tids_GasAnalysis_Reading where
-" tids_GasAnalysis_Reading = 
-    (filter 
-        (\<lambda> s. s \<notin> {NULLTRANSITION__GasAnalysis, TID_GasAnalysis_t9a,
-          TID_GasAnalysis_t8, TID_GasAnalysis_t4, TID_GasAnalysis_t3, 
-          TID_GasAnalysis_t2, TID_GasAnalysis_t0}) 
-        ITIDS_GasAnalysis_list)"
-
-abbreviation Other_SIDs_to_Reading_GasAnalysis where
-"Other_SIDs_to_Reading_GasAnalysis \<equiv>
-  set [(s, SID_GasAnalysis_Reading) . s \<leftarrow> (SIDS_GasAnalysis_no_Reading)]"
-
-definition State_GasAnalysis_Reading where 
-"State_GasAnalysis_Reading = 
-  loop (\<lambda> (id::integer).
-    do {sd \<leftarrow> inp_in enter_GasAnalysis Other_SIDs_to_Reading_GasAnalysis ; 
-        \<comment> \<open> State passed to next loop, including a condition initially True. \<close>
-        ret \<leftarrow> Ret (True, id, fst sd) ; 
-        \<comment> \<open> State_GasAnalysis_Reading_execute \<close>
-        (iterate 
-           \<comment> \<open> condition \<close>
-           (\<lambda> s. fst s) 
-           \<comment> \<open> P \<close>
-           (\<lambda> s.
-            do {
-              outp entered_GasAnalysis (snd (snd s), SID_GasAnalysis_Reading);
-              (do {skip ; stop} \<triangle>
-                (
-                \<comment> \<open> T_GasAnalysis_t0 \<close>
-                do {gs \<leftarrow> inp_in gas__GasAnalysis (set [(TID_GasAnalysis_t0, din, x). 
-                        x \<leftarrow> (lseq_gassensor_enum)]) ;
-                    outp set_gs_GasAnalysis (snd (snd gs));
-                    outp exit_GasAnalysis (SID_GasAnalysis_Reading, SID_GasAnalysis_Reading);
-                    outp exited_GasAnalysis (SID_GasAnalysis_Reading, SID_GasAnalysis_Reading);
-                    outp enter_GasAnalysis (SID_GasAnalysis_Reading, SID_GasAnalysis_Analysis);
-                    outp entered_GasAnalysis (SID_GasAnalysis_Reading, SID_GasAnalysis_Analysis);
-                    Ret(False, fst (snd s), SID_GasAnalysis_Reading)
-                    } \<box>
-                (exit_events_GasAnalysis (fst (snd s)) SID_GasAnalysis_Reading 
-                   tids_GasAnalysis_Reading Other_SIDs_to_Reading_GasAnalysis)
-                )
-              )
-            })
-            \<comment> \<open> The previous state: a triple \<close> 
-            (ret)
-        ) ;
-        Ret (id)
-  }
-)
-"
-
-definition State_GasAnalysis_Reading_R where
-"State_GasAnalysis_Reading_R (idd::integer) = 
-   (discard_state (State_GasAnalysis_Reading idd)) \<comment> \<open> discard state to match with skip on the right\<close>
-    \<parallel>\<^bsub> (int_int_GasAnalysis - GasAnalysis_Reading_triggers) \<^esub> 
-   skip
-"
-
-subsubsection \<open> State machine \<close>
-definition flow_events_GasAnalysis_stm_to_nodes where
-"flow_events_GasAnalysis_stm_to_nodes = (
- let nodes = [SID_GasAnalysis_NoGas,SID_GasAnalysis_Analysis,SID_GasAnalysis_GasDetected,
-              SID_GasAnalysis_j1,SID_GasAnalysis_Reading]
- in set (
-      enumchans2 [enter_GasAnalysis_C, entered_GasAnalysis_C,exit_GasAnalysis_C,exited_GasAnalysis_C] 
-          (filter (\<lambda> s. s \<notin> set nodes) SIDS_GasAnalysis_list) nodes
-  )
-)"
-
-definition STM_GasAnalysis where
-"STM_GasAnalysis (idd::integer) = 
-   (I_GasAnalysis_i1(idd))
-    \<parallel>\<^bsub> flow_events_GasAnalysis_stm_to_nodes \<^esub> 
-   (State_GasAnalysis_NoGas_R(idd)
-      \<parallel>\<^bsub> CS_GasAnalysis_Analysis_sync \<inter> (CS_GasAnalysis_Analysis_sync \<union> 
-          (CS_GasAnalysis_GasDetected_sync \<union> (CS_GasAnalysis_j1_sync \<union> CS_GasAnalysis_Reading_sync))) \<^esub>
-      (State_GasAnalysis_Analysis_R(idd)
-        \<parallel>\<^bsub> CS_GasAnalysis_Analysis_sync \<inter> (CS_GasAnalysis_GasDetected_sync \<union> 
-            (CS_GasAnalysis_j1_sync \<union> CS_GasAnalysis_Reading_sync)) \<^esub> 
-        ( State_GasAnalysis_GasDetected_R(idd)
-          \<parallel>\<^bsub> CS_GasAnalysis_GasDetected_sync \<inter> (CS_GasAnalysis_j1_sync \<union> CS_GasAnalysis_Reading_sync) \<^esub> 
-          (State_GasAnalysis_j1_R(idd)  
-            \<parallel>\<^bsub> CS_GasAnalysis_j1_sync \<inter> CS_GasAnalysis_Reading_sync \<^esub> 
-          State_GasAnalysis_Reading_R(idd))
-        )
-      )
-   )
-"
-
-definition GasAnalysis_opt_0_internal_set where
-"GasAnalysis_opt_0_internal_set = 
-  set (([internal_GasAnalysis_C TID_GasAnalysis_t1]) @ 
-       (enumchans3 [gas__GasAnalysis_C] 
-          [TID_GasAnalysis_t0, TID_GasAnalysis_t2] 
-          [din, dout] 
-          (lseq_gassensor_enum))
-)"
-
-definition GasAnalysis_opt_1_internal_set where
-"GasAnalysis_opt_1_internal_set = 
-  set ((enumchans1 [internal_GasAnalysis_C] [TID_GasAnalysis_t4, TID_GasAnalysis_t3]) @
-       (enumchans1 [set_st_GasAnalysis_C] Chemical_Status_list)
-)"
-
-definition GasAnalysis_opt_2_internal_set where
-"GasAnalysis_opt_2_internal_set = 
-  set ((enumchans1 [internal_GasAnalysis_C] [TID_GasAnalysis_t8, TID_GasAnalysis_t9a])
-)"
-
-definition MemorySTM_opt_GasAnalysis where
-"MemorySTM_opt_GasAnalysis (idd::integer) = 
-  (par_hide
-    (discard_state (GasAnalysis_Memory_opt_i (Chemical_IntensityC (0::2))))
-    GasAnalysis_i_events
-    (par_hide 
-      (par_hide
-        (discard_state (GasAnalysis_Memory_opt_st (Chemical_Status_noGas)))
-        GasAnalysis_st_events
-        (hide 
-          (
-            (hide
-              (
-                (par_hide
-                  (discard_state (GasAnalysis_Memory_opt_gs (bmake TYPE(2) [])))
-                  GasAnalysis_gs_events
-                  (par_hide 
-                    (discard_state (GasAnalysis_Memory_opt_a Chemical_Angle_Left)) 
-                    GasAnalysis_a_events 
-                    (STM_GasAnalysis idd)
-                  )
-                )
-                \<parallel>\<^bsub> GasAnalysis_opt_0_internal_set \<^esub>
-                (discard_state (GasAnalysis_MemoryTransitions_opt_0 idd))
-              )
-              ({internal_GasAnalysis_C TID_GasAnalysis_t1})
-            )
-            \<parallel>\<^bsub> GasAnalysis_opt_1_internal_set \<^esub> 
-            (discard_state (GasAnalysis_MemoryTransitions_opt_1 idd))
-          )
-          (set (enumchans1 [internal_GasAnalysis_C] [TID_GasAnalysis_t4, TID_GasAnalysis_t3]))
-        )
-      )
-      GasAnalysis_opt_2_internal_set
-      (discard_state (GasAnalysis_MemoryTransitions_opt_2 idd))
-    )
-  )   
-"
-
-definition rename_GasAnalysis_events where
-"rename_GasAnalysis_events = 
-  concat (
-    (enumchan2 (forget_first2 gas__GasAnalysis_C gas_GasAnalysis_C TIDS_GasAnalysis_list) 
-            InOut_list lseq_gassensor_enum) @
-    (enumchan2 (forget_first2 turn__GasAnalysis_C turn_GasAnalysis_C TIDS_GasAnalysis_list) 
-            InOut_list Chemical_Angle_list) @
-    (enumchan1 (forget_first resume__GasAnalysis_C resume_GasAnalysis_C TIDS_GasAnalysis_list) 
-            InOut_list) @
-    (enumchan1 (forget_first stop__GasAnalysis_C stop_GasAnalysis_C TIDS_GasAnalysis_list) 
-            InOut_list)
-  )
-"
-
-term "\<lbrace>resume__GasAnalysis (t, x) \<mapsto> resume_GasAnalysis x | x. x \<in> InOut_set\<rbrace>"
-term "\<lbrace>terminate_GasAnalysis () \<mapsto> terminate_GasAnalysis () | _. True\<rbrace>"
-
-definition rename_GasAnalysis_events_others where
-"rename_GasAnalysis_events_others = 
-  (enumchanp1 terminate_GasAnalysis_C [()]) @
-  (enumchansp1 [get_i_GasAnalysis_C, set_i_GasAnalysis_C] Chemical_Intensity2_list) @
-  (enumchansp1 [get_a_GasAnalysis_C, set_a_GasAnalysis_C] Chemical_Angle_list) @
-  (enumchansp1 [get_st_GasAnalysis_C, set_st_GasAnalysis_C] Chemical_Status_list) @
-  (enumchansp1 [get_gs_GasAnalysis_C, set_gs_GasAnalysis_C] lseq_gassensor_enum) @
-  (enumchansp2 [gas_GasAnalysis_C] InOut_list lseq_gassensor_enum) @
-  (enumchansp2 [turn_GasAnalysis_C] InOut_list Chemical_Angle_list) @
-  (enumchansp1 [resume_GasAnalysis_C, stop_GasAnalysis_C] InOut_list) @
-  (enumchansp2 [enter_GasAnalysis_C, entered_GasAnalysis_C, exit_GasAnalysis_C, exited_GasAnalysis_C] 
-    SIDS_GasAnalysis_list SIDS_GasAnalysis_list) @
-  (enumchansp1 [internal_GasAnalysis_C] TIDS_GasAnalysis_list)
-"
-
-definition rename_MemorySTM_opt_GasAnalysis where
-"rename_MemorySTM_opt_GasAnalysis idd = 
-  rename (set (rename_GasAnalysis_events @ rename_GasAnalysis_events_others)) 
-    (MemorySTM_opt_GasAnalysis idd)
-"
-
-definition AUX_opt_GasAnalysis where
-"AUX_opt_GasAnalysis (idd::integer) = 
-  (hide 
-    ( 
-      (rename_MemorySTM_opt_GasAnalysis idd) \<lbrakk> set [terminate_GasAnalysis_C ()] \<Zrres> skip
-    )
-    GasAnalysis_MachineInternalEvents
-  )
-"
-
-definition D__GasAnalysis where
-"D__GasAnalysis (idd::integer) = 
-  hide (AUX_opt_GasAnalysis idd) internal_events_GasAnalysis
-"
-
-subsection \<open> MainController \<close>
-chantype Chan_MainCtrl =
-  terminate_MainCtrl :: unit
-  gas_MainCtrl :: "InOut \<times> 2 Chemical_GasSensor[2]blist"
-  resume_MainCtrl :: "InOut"
-  turn_MainCtrl :: "InOut \<times> Chemical_Angle"
-  stop_MainCtrl :: "InOut"
-
-subsubsection \<open> Memory \<close>
-definition Memory_MainCtrl where
-"Memory_MainCtrl (idd::integer) = skip"
-
-subsubsection \<open> Controller \<close>
-
-definition rename_MainCtrl_GasAnalysis_events where
-"rename_MainCtrl_GasAnalysis_events = 
-  (enumchanp2_1 (terminate_GasAnalysis_C,terminate_MainCtrl_C) [()]) @
-  (enumchansp2_2 [(gas_GasAnalysis_C, gas_MainCtrl_C)] InOut_list lseq_gassensor_enum) @
-  (enumchansp2_1 [(resume_GasAnalysis_C, resume_MainCtrl_C)] InOut_list) @
-  (enumchansp2_2 [(turn_GasAnalysis_C, turn_MainCtrl_C)] InOut_list Chemical_Angle_list) @
-  (enumchansp2_1 [(stop_GasAnalysis_C, stop_MainCtrl_C)] InOut_list)
-"
-
-definition rename_D__GasAnalysis where
-  "rename_D__GasAnalysis idd = rename (set rename_MainCtrl_GasAnalysis_events) (D__GasAnalysis idd)"
-
-definition D__MainCtrl where
-"D__MainCtrl (idd::integer) = 
-  (par_hide
-    (rename_D__GasAnalysis idd)
-    {}
-    (discard_state (Memory_MainCtrl idd))
-  )  \<lbrakk> set [terminate_MainCtrl_C ()] \<Zrres> skip
-"
 
 subsection \<open> Movement \<close>
 subsubsection \<open> Constants \<close>
@@ -1022,7 +48,9 @@ definition "SIDS_Movement_no_TryingAgain = (removeAll SID_Movement_TryingAgain S
 definition "SIDS_Movement_no_AvoidingAgain = (removeAll SID_Movement_AvoidingAgain SIDS_Movement_list)"
 definition "SIDS_Movement_no_GettingOut = (removeAll SID_Movement_GettingOut SIDS_Movement_list)"
 
-enumtype TIDS_Movement = NULLTRANSITION__Movement
+(* Here we change enumtype to datatype as enumtype will take very long time to resolve 
+this definition (I mean Isabelle keeps running poly and high CPU usage.) *)
+datatype TIDS_Movement = NULLTRANSITION__Movement
 	              | TID_Movement_t1
 	              | TID_Movement_t2
 	              | TID_Movement_t3
@@ -1046,8 +74,16 @@ enumtype TIDS_Movement = NULLTRANSITION__Movement
 	              | TID_Movement_t22
 	              | TID_Movement_t13
 	              | TID_Movement_t5
-
+(*
 definition "TIDS_Movement_list = enum_TIDS_Movement_inst.enum_TIDS_Movement"
+*)
+definition "TIDS_Movement_list = [NULLTRANSITION__Movement, TID_Movement_t0,
+  TID_Movement_t1, TID_Movement_t2, TID_Movement_t3, TID_Movement_t4, TID_Movement_t5,
+  TID_Movement_t6, TID_Movement_t7, TID_Movement_t8, TID_Movement_t9, TID_Movement_t10, 
+  TID_Movement_t11, TID_Movement_t12, TID_Movement_t13, TID_Movement_t14, TID_Movement_t15, 
+  TID_Movement_t16, TID_Movement_t17, TID_Movement_t18, TID_Movement_t19, TID_Movement_t20, 
+  TID_Movement_t21, TID_Movement_t22]"
+
 definition "TIDS_Movement_set = set TIDS_Movement_list"
 
 text \<open> Identifiers of transitions that can interrupt a state, excluding transitions from junctions. \<close>
@@ -1081,246 +117,272 @@ chantype Chan_Movement =
   set_a_Movement :: "Chemical_Angle"
 
 (* event channels *)
-  gas__Movement :: "TIDS_Movement \<times> InOut \<times> 2 Chemical_GasSensor[2]blist"
-  gas_Movement :: "InOut \<times> 2 Chemical_GasSensor[2]blist"
+  obstacle__Movement :: "TIDS_Movement \<times> InOut \<times> Location_Loc"
+  obstacle_Movement :: "InOut \<times> Location_Loc"
+  odometer__Movement :: "TIDS_Movement \<times> InOut \<times> core_real"
+  odometer_Movement :: "InOut \<times> core_real"
   resume__Movement :: "TIDS_Movement \<times> InOut"
   resume_Movement :: "InOut"
   turn__Movement :: "TIDS_Movement \<times> InOut \<times> Chemical_Angle"
   turn_Movement :: "InOut \<times> Chemical_Angle"
   stop__Movement :: "TIDS_Movement \<times> InOut"
   stop_Movement :: "InOut"
+  flag__Movement :: "TIDS_Movement \<times> InOut"
+  flag_Movement :: "InOut"
+
+(* Call events for undefined operations *)
+  changeDirectionCall_Movement :: "Location_Loc"
+  randomeWalkCall_Movement :: unit
+  moveCall :: "core_real \<times> Chemical_Angle"
+  shortRandomWalkCall :: unit
 
 subsubsection \<open> Sets of events \<close>
-(* How to use a list to represent all possible values of Chemical_GasSensor[2]blist *)
+
+abbreviation "int_int_tids_Movement \<equiv> 
+  removeAll NULLTRANSITION__Movement (removeAll (TID_Movement_t1) TIDS_Movement_list)"
+(*[TID_Movement_t0,
+  TID_Movement_t2, TID_Movement_t3, TID_Movement_t4, TID_Movement_t5,
+  TID_Movement_t6, TID_Movement_t7, TID_Movement_t8, TID_Movement_t9, TID_Movement_t10, 
+  TID_Movement_t11, TID_Movement_t12, TID_Movement_t13, TID_Movement_t14, TID_Movement_t15, 
+  TID_Movement_t16, TID_Movement_t17, TID_Movement_t18, TID_Movement_t19, TID_Movement_t20, 
+  TID_Movement_t21, TID_Movement_t22]*)
+
 definition int_int_Movement where
 "int_int_Movement = set (
-  (enumchans3 [gas__Movement_C] 
-    [TID_Movement_t0, TID_Movement_t2, 
-     TID_Movement_t3, TID_Movement_t4,
-     TID_Movement_t8, TID_Movement_t9a] 
-    [din, dout] 
-    (lseq_gassensor_enum)) @
-  (enumchans2 [resume__Movement_C] 
-    [TID_Movement_t0, TID_Movement_t2, 
-     TID_Movement_t3, TID_Movement_t4,
-     TID_Movement_t8, TID_Movement_t9a] 
-    [din, dout]) @
-  (enumchans3 [turn__Movement_C] 
-    [TID_Movement_t0, TID_Movement_t2, 
-     TID_Movement_t3, TID_Movement_t4,
-     TID_Movement_t8, TID_Movement_t9a] 
-    [din, dout]
-    Chemical_Angle_list
-    ) @
-  (enumchans2 [stop__Movement_C] 
-    [TID_Movement_t0, TID_Movement_t2, 
-     TID_Movement_t3, TID_Movement_t4,
-     TID_Movement_t8, TID_Movement_t9a] 
-    [din, dout]  
-    ) @
-  (enumchan1 internal_Movement_C 
-    [TID_Movement_t0, TID_Movement_t2, 
-     TID_Movement_t3, TID_Movement_t4,
-     TID_GasAnalysis_t8, TID_GasAnalysis_t9a])
+  (enumchans3 [obstacle__Movement_C] int_int_tids_Movement [din, dout] Location_Loc_list) @
+  (enumchans3 [odometer__Movement_C] int_int_tids_Movement [din, dout] rc.core_real_list) @
+  (enumchans2 [resume__Movement_C, stop__Movement_C, flag__Movement_C] 
+    int_int_tids_Movement [din, dout]) @
+  (enumchans3 [turn__Movement_C] int_int_tids_Movement [din, dout] Chemical_Angle_list) @
+  (enumchan1 internal_Movement_C int_int_tids_Movement)
 )"
 
-abbreviation "enter_exit_channels_GasAnalysis \<equiv>
-  [enter_GasAnalysis_C, entered_GasAnalysis_C, exit_GasAnalysis_C, exited_GasAnalysis_C]"
+abbreviation "enter_exit_channels_Movement \<equiv>
+  [enter_Movement_C, entered_Movement_C, exit_Movement_C, exited_Movement_C]"
 
-definition internal_events_GasAnalysis where
-"internal_events_GasAnalysis = set (
-  enumchans2 enter_exit_channels_GasAnalysis SIDS_GasAnalysis_list SIDS_GasAnalysis_list
+definition internal_events_Movement where
+"internal_events_Movement = set (
+  enumchans2 enter_exit_channels_Movement SIDS_Movement_list SIDS_Movement_list
 )"
 
 
-definition GasAnalysis_i_events where
-"GasAnalysis_i_events = 
-    set (enumchans1 [get_i_GasAnalysis_C, set_i_GasAnalysis_C] Chemical_Intensity2_list)
+definition Movement_d0_events where
+"Movement_d0_events = 
+    set (enumchans1 [get_d0_Movement_C, set_d0_Movement_C] rc.core_real_list)
 "
 
-definition GasAnalysis_st_events where
-"GasAnalysis_st_events = 
-    set (enumchans1 [get_st_GasAnalysis_C, set_st_GasAnalysis_C] Chemical_Status_list)
+definition Movement_d1_events where
+"Movement_d1_events = 
+    set (enumchans1 [get_d1_Movement_C, set_d1_Movement_C] rc.core_real_list)
 "
 
-definition GasAnalysis_gs_events where
-"GasAnalysis_gs_events = 
-    set (enumchans1 [get_gs_GasAnalysis_C, set_gs_GasAnalysis_C] lseq_gassensor_enum)
+definition Movement_l_events where
+"Movement_l_events = 
+    set (enumchans1 [get_l_Movement_C, set_l_Movement_C] Location_Loc_list)
 "
 
-definition GasAnalysis_a_events where
-"GasAnalysis_a_events = 
-    set (enumchans1 [get_a_GasAnalysis_C, set_a_GasAnalysis_C] Chemical_Angle_list)
+definition Movement_a_events where
+"Movement_a_events = 
+    set (enumchans1 [get_a_Movement_C, set_a_Movement_C] Chemical_Angle_list)
 "
 
-definition GasAnalysis_MachineInternalEvents where
-"GasAnalysis_MachineInternalEvents = 
-  set (enumchan1 internal_GasAnalysis_C TIDS_GasAnalysis_list)
+definition Movement_MachineInternalEvents where
+"Movement_MachineInternalEvents = 
+  set (enumchan1 internal_Movement_C TIDS_Movement_list)
 "
 
 subsubsection \<open> State Machine Memory \<close>
 text \<open> Memory cell processes \<close>
 
 (* for the local variable x *)
-definition GasAnalysis_Memory_opt_gs where
-"GasAnalysis_Memory_opt_gs = 
-  mem_of_lvar get_gs_GasAnalysis set_gs_GasAnalysis 
-    (set (lseq_gassensor_enum))"
+definition Movement_Memory_opt_d0 where
+"Movement_Memory_opt_d0 = 
+  mem_of_lvar get_d0_Movement set_d0_Movement (rc.core_real_set)"
 
-definition GasAnalysis_Memory_opt_a where
-"GasAnalysis_Memory_opt_a = mem_of_lvar get_a_GasAnalysis set_a_GasAnalysis Chemical_Angle_set"
+definition Movement_Memory_opt_d1 where
+"Movement_Memory_opt_d1 = 
+  mem_of_lvar get_d1_Movement set_d1_Movement (rc.core_real_set)"
 
-definition GasAnalysis_Memory_opt_i where
-"GasAnalysis_Memory_opt_i = mem_of_lvar get_i_GasAnalysis set_i_GasAnalysis (Chemical_Intensity2_set)"
+definition Movement_Memory_opt_a where
+"Movement_Memory_opt_a = mem_of_lvar get_a_Movement set_a_Movement Chemical_Angle_set"
 
-definition GasAnalysis_Memory_opt_st where
-"GasAnalysis_Memory_opt_st = mem_of_lvar get_st_GasAnalysis set_st_GasAnalysis (Chemical_Status_set)"
+definition Movement_Memory_opt_l where
+"Movement_Memory_opt_l = mem_of_lvar get_l_Movement set_l_Movement (Location_Loc_set)"
 
 text \<open> Memory transition processes \<close>
-definition GasAnalysis_MemoryTransitions_opt_0 where
-"GasAnalysis_MemoryTransitions_opt_0 = 
+definition Movement_MemoryTransitions_opt_0 where
+"Movement_MemoryTransitions_opt_0 = 
   loop (\<lambda> id::integer. 
-    (do {outp internal_GasAnalysis TID_GasAnalysis_t1 ; Ret (id)} \<box> 
-     do {gs \<leftarrow> inp_in gas__GasAnalysis (set [(TID_GasAnalysis_t2, din, x). 
-              x \<leftarrow> (lseq_gassensor_enum)]) ; Ret (id)}  \<box> 
-     do {gs \<leftarrow> inp_in gas__GasAnalysis (set [(TID_GasAnalysis_t0, din, x). 
-              x \<leftarrow> (lseq_gassensor_enum)]) ; Ret (id)})
-  )
+    ( 
+    do {outp resume__Movement (TID_Movement_t0, din) ; Ret (id)} \<box> 
+    do {a \<leftarrow> inp_in turn__Movement (set [(TID_Movement_t3, din, x). 
+              x \<leftarrow> (Chemical_Angle_list)]) ; Ret (id)} \<box> 
+    do {outp stop__Movement (TID_Movement_t16, din) ; Ret (id)} \<box>
+    do {outp stop__Movement (TID_Movement_t17, din) ; Ret (id)} \<box> 
+    do {a \<leftarrow> inp_in turn__Movement (set [(TID_Movement_t14, din, x). 
+              x \<leftarrow> (Chemical_Angle_list)]) ; Ret (id)} \<box> 
+    do {outp resume__Movement (TID_Movement_t22, din) ; Ret (id)} \<box> 
+    do {outp stop__Movement (TID_Movement_t18, din) ; Ret (id)} \<box>
+    do {outp resume__Movement (TID_Movement_t20, din) ; Ret (id)} \<box>
+    do {outp internal_Movement TID_Movement_t1 ; Ret (id)} \<box>
+    do {l \<leftarrow> inp_in obstacle__Movement (set [(TID_Movement_t6, din, l). 
+              l \<leftarrow> (Location_Loc_list)]) ; Ret (id)} \<box>
+    do {outp resume__Movement (TID_Movement_t21, din) ; Ret (id)} \<box>
+    do {outp stop__Movement (TID_Movement_t15, din) ; Ret (id)} \<box>
+    do {outp internal_Movement TID_Movement_t5 ; Ret (id)} \<box>
+    do {outp stop__Movement (TID_Movement_t4, din) ; Ret (id)} \<box>
+    do {outp resume__Movement (TID_Movement_t10, din) ; Ret (id)} \<box>
+    do {a \<leftarrow> inp_in turn__Movement (set [(TID_Movement_t7, din, x). 
+              x \<leftarrow> (Chemical_Angle_list)]) ; Ret (id)} \<box> 
+    do {outp stop__Movement (TID_Movement_t9, din) ; Ret (id)} \<box>
+    do {outp resume__Movement (TID_Movement_t19, din) ; Ret (id)} \<box>
+    do {l \<leftarrow> inp_in obstacle__Movement (set [(TID_Movement_t11, din, l). 
+              l \<leftarrow> (Location_Loc_list)]) ; Ret (id)} \<box>
+    do {a \<leftarrow> inp_in turn__Movement (set [(TID_Movement_t8, din, x). 
+              x \<leftarrow> (Chemical_Angle_list)]) ; Ret (id)} \<box> 
+    do {a \<leftarrow> inp_in turn__Movement (set [(TID_Movement_t2, din, x). 
+              x \<leftarrow> (Chemical_Angle_list)]) ; Ret (id)}
+    )
+)
 "
 
-definition GasAnalysis_MemoryTransitions_opt_1 where
-"GasAnalysis_MemoryTransitions_opt_1 = 
+definition Movement_MemoryTransitions_opt_1 where
+"Movement_MemoryTransitions_opt_1 = 
   loop (\<lambda> id::integer.
-    do {st \<leftarrow> inp_in get_st_GasAnalysis Chemical_Status_set ; 
-      (
-        do {guard (st = Chemical_Status_gasD); outp internal_GasAnalysis TID_GasAnalysis_t4 ; Ret (id)} \<box>
-        do {guard (st = Chemical_Status_noGas); outp internal_GasAnalysis TID_GasAnalysis_t3 ; Ret (id)} \<box>
-        do {x \<leftarrow> inp_in set_st_GasAnalysis Chemical_Status_set; Ret (id)}
-      )
-    }
-  )
-"
-
-definition GasAnalysis_MemoryTransitions_opt_2 where
-"GasAnalysis_MemoryTransitions_opt_2 = 
-  loop (\<lambda> id::integer.
-    do {i \<leftarrow> inp_in get_i_GasAnalysis Chemical_Intensity2_set ; 
-      (
-        do {guard (\<not> (Chemical_goreq i const_GasAnalysis_thr)); outp internal_GasAnalysis TID_GasAnalysis_t9a ; Ret (id)} \<box>
-        do {guard (Chemical_goreq i const_GasAnalysis_thr); outp internal_GasAnalysis TID_GasAnalysis_t8 ; Ret (id)} \<box>
-        do {x \<leftarrow> inp_in set_i_GasAnalysis Chemical_Intensity2_set; Ret (id)}
-      )
+    do {d1 \<leftarrow> inp_in get_d1_Movement rc.core_real_set ; 
+        d0 \<leftarrow> inp_in get_d0_Movement rc.core_real_set ;
+        (
+          do {guard (True); outp internal_Movement TID_Movement_t12 ; Ret (id)} \<box>
+          do {guard (True); outp internal_Movement TID_Movement_t13 ; Ret (id)} \<box>
+          do {inp_in set_d1_Movement rc.core_real_set; Ret (id)} \<box>
+          do {inp_in set_d0_Movement rc.core_real_set; Ret (id)}
+        )
     }
   )
 "
 
 subsubsection \<open> States \<close>
 paragraph \<open> Initial \<close>
-definition I_GasAnalysis_i1 where
-"I_GasAnalysis_i1 = (\<lambda> (id::integer) . 
-  do {outp internal_GasAnalysis TID_GasAnalysis_t1 ; 
-      outp enter_GasAnalysis (SID_GasAnalysis, SID_GasAnalysis_NoGas);
-      outp entered_GasAnalysis (SID_GasAnalysis, SID_GasAnalysis_NoGas)
+definition I_Movement_i1 where
+"I_Movement_i1 = (\<lambda> (id::integer) . 
+  do {outp internal_Movement TID_Movement_t1 ; 
+      outp enter_Movement (SID_Movement, SID_Movement_Waiting);
+      outp entered_Movement (SID_Movement, SID_Movement_Waiting)
   })
 "
 
-paragraph \<open> NoGas \<close>
-definition CS_GasAnalysis_NoGas_sync where
-"CS_GasAnalysis_NoGas_sync = 
+paragraph \<open> Waiting \<close>
+definition CS_Movement_Waiting_sync where
+"CS_Movement_Waiting_sync = 
   set (
       \<comment> \<open> enter from x to y \<close>
-      (enumchans2 enter_exit_channels_GasAnalysis [SID_GasAnalysis_NoGas] SIDS_GasAnalysis_nodes)@
+      (enumchans2 enter_exit_channels_Movement [SID_Movement_Waiting] SIDS_Movement_nodes)@
       \<comment> \<open> enter from y to x \<close>
-      (enumchans2 enter_exit_channels_GasAnalysis SIDS_GasAnalysis_nodes [SID_GasAnalysis_NoGas])
+      (enumchans2 enter_exit_channels_Movement SIDS_Movement_nodes [SID_Movement_Waiting])
 )"
 
-definition GasAnalysis_NoGas_triggers where
-"GasAnalysis_NoGas_triggers = set (
-  (enumchan1 internal_GasAnalysis_C 
-    [TID_GasAnalysis_t3, TID_GasAnalysis_t4,
-     TID_GasAnalysis_t8, TID_GasAnalysis_t9a]) @
-  (enumchans3 [gas__GasAnalysis_C] 
-    [TID_GasAnalysis_t0, TID_GasAnalysis_t2] 
-    [din, dout] 
-    (lseq_gassensor_enum))
+definition Movement_Waiting_triggers where
+"Movement_Waiting_triggers = set (
+  (enumchans3 [obstacle__Movement_C] [TID_Movement_t6, TID_Movement_t11] [din, dout] Location_Loc_list) @
+  (enumchans2 [resume__Movement_C] 
+    [TID_Movement_t0, TID_Movement_t22, TID_Movement_t20, TID_Movement_t21, TID_Movement_t10, 
+    TID_Movement_t19] [din, dout]) @
+  (enumchans2 [stop__Movement_C] 
+    [TID_Movement_t16, TID_Movement_t17, TID_Movement_t18, TID_Movement_t15, TID_Movement_t4, 
+    TID_Movement_t9] [din, dout]) @
+  (enumchans3 [turn__Movement_C] [TID_Movement_t3, TID_Movement_t14, TID_Movement_t7, 
+    TID_Movement_t8, TID_Movement_t2] [din, dout] Chemical_Angle_list) @
+  (enumchan1 internal_Movement_C [TID_Movement_t12, TID_Movement_t5, TID_Movement_t13])
 )
 "
 
-definition tids_GasAnalysis_NoGas where
-" tids_GasAnalysis_NoGas = 
+(* empty list *)
+definition tids_Movement_Waiting where
+" tids_Movement_Waiting = 
     (filter 
-        (\<lambda> s. s \<notin> {NULLTRANSITION__GasAnalysis, TID_GasAnalysis_t9a,
-          TID_GasAnalysis_t8, TID_GasAnalysis_t4, TID_GasAnalysis_t3, 
-          TID_GasAnalysis_t2, TID_GasAnalysis_t0}) 
-        ITIDS_GasAnalysis_list)"
+        (\<lambda> s. s \<notin> (set ITIDS_Movement_list)) 
+        ITIDS_Movement_list)"
 
-abbreviation Other_SIDs_to_NoGas_GasAnalysis where
-"Other_SIDs_to_NoGas_GasAnalysis \<equiv>
-  set [(s, SID_GasAnalysis_NoGas) . s \<leftarrow> (SIDS_GasAnalysis_no_NoGas)]"
+abbreviation Other_SIDs_to_Waiting_Movement where
+"Other_SIDs_to_Waiting_Movement \<equiv>
+  set [(s, SID_Movement_Waiting) . s \<leftarrow> (SIDS_Movement_no_Waiting)]"
 
 definition 
-"exit_events_GasAnalysis idd sid tids other_sids =
-    (do {inp_in internal_GasAnalysis (set tids);
-        y \<leftarrow> inp_in exit_GasAnalysis other_sids;
-          outp exited_GasAnalysis (fst y, sid);
+"exit_events_Movement idd sid tids other_sids =
+    (do {inp_in internal_Movement (set tids);
+        y \<leftarrow> inp_in exit_Movement other_sids;
+          outp exited_Movement (fst y, sid);
           Ret(False, idd, sid)
         } \<box>
-    do {t \<leftarrow> inp_in gas__GasAnalysis (set [(t, d, gs). 
+    do {r \<leftarrow> inp_in obstacle__Movement (set [(t, d, l). 
             t \<leftarrow> (tids), d \<leftarrow> InOut_list,
-            gs \<leftarrow> (lseq_gassensor_enum)]) ;
-          y \<leftarrow> inp_in exit_GasAnalysis other_sids;
-            outp exited_GasAnalysis (fst y, sid);
+            l \<leftarrow> (Location_Loc_list)]) ;
+          y \<leftarrow> inp_in exit_Movement other_sids;
+            outp exited_Movement (fst y, sid);
             Ret(False, idd, sid)
         } \<box>
-    do {t \<leftarrow> inp_in resume__GasAnalysis (set [(t, d). 
+    do {r \<leftarrow> inp_in odometer__Movement (set [(t, d, l). 
+            t \<leftarrow> (tids), d \<leftarrow> InOut_list,
+            l \<leftarrow> rc.core_real_list]) ;
+          y \<leftarrow> inp_in exit_Movement other_sids;
+            outp exited_Movement (fst y, sid);
+            Ret(False, idd, sid)
+        } \<box>
+    do {t \<leftarrow> inp_in resume__Movement (set [(t, d). 
             t \<leftarrow> (tids), d \<leftarrow> InOut_list]) ;
-          y \<leftarrow> inp_in exit_GasAnalysis other_sids;
-            outp exited_GasAnalysis (fst y, sid);
+          y \<leftarrow> inp_in exit_Movement other_sids;
+            outp exited_Movement (fst y, sid);
             Ret(False, idd, sid)
         } \<box>
-    do {t \<leftarrow> inp_in turn__GasAnalysis (set [(t, d, a). 
+    do {t \<leftarrow> inp_in turn__Movement (set [(t, d, a). 
             t \<leftarrow> (tids), d \<leftarrow> InOut_list,
             a \<leftarrow> Chemical_Angle_list]) ;
-          y \<leftarrow> inp_in exit_GasAnalysis other_sids;
-            outp exited_GasAnalysis (fst y, sid);
+          y \<leftarrow> inp_in exit_Movement other_sids;
+            outp exited_Movement (fst y, sid);
             Ret(False, idd, sid)
         } \<box>
-    do {t \<leftarrow> inp_in stop__GasAnalysis (set [(t, d). 
+    do {t \<leftarrow> inp_in stop__Movement (set [(t, d). 
             t \<leftarrow> (tids), d \<leftarrow> InOut_list]) ;
-          y \<leftarrow> inp_in exit_GasAnalysis other_sids;
-            outp exited_GasAnalysis (fst y, sid);
+          y \<leftarrow> inp_in exit_Movement other_sids;
+            outp exited_Movement (fst y, sid);
+            Ret(False, idd, sid)
+        } \<box>
+    do {t \<leftarrow> inp_in flag__Movement (set [(t, d). 
+            t \<leftarrow> (tids), d \<leftarrow> InOut_list]) ;
+          y \<leftarrow> inp_in exit_Movement other_sids;
+            outp exited_Movement (fst y, sid);
             Ret(False, idd, sid)
         }
     )"
 
-definition State_GasAnalysis_NoGas where 
-"State_GasAnalysis_NoGas = 
+definition State_Movement_Waiting where 
+"State_Movement_Waiting = 
   loop (\<lambda> (id::integer).
-    do {sd \<leftarrow> inp_in enter_GasAnalysis Other_SIDs_to_NoGas_GasAnalysis ; 
+    do {sd \<leftarrow> inp_in enter_Movement Other_SIDs_to_Waiting_Movement ; 
         \<comment> \<open> State passed to next loop, including a condition initially True. \<close>
         ret \<leftarrow> Ret (True, id, fst sd) ; 
-        \<comment> \<open> State_GasAnalysis_NoGas_execute \<close>
+        \<comment> \<open> State_Movement_Waiting_execute \<close>
         (iterate 
            \<comment> \<open> condition \<close>
            (\<lambda> s. fst s) 
            \<comment> \<open> P \<close>
            (\<lambda> s.
             do {
-              outp entered_GasAnalysis (snd (snd s), SID_GasAnalysis_NoGas);
+              outp entered_Movement (snd (snd s), SID_Movement_Waiting);
               (do {skip ; stop} \<triangle>
                 (
-                \<comment> \<open> T_GasAnalysis_t2 \<close>
-                do {t \<leftarrow> inp_in gas__GasAnalysis (set [(TID_GasAnalysis_t2, din, gs). 
+                \<comment> \<open> T_Movement_t2 \<close>
+                do {t \<leftarrow> inp_in gas__Movement (set [(TID_Movement_t2, din, gs). 
                                 gs \<leftarrow> (lseq_gassensor_enum)]) ;
-                      outp set_gs_GasAnalysis (snd (snd t)) ; 
-                      outp exit_GasAnalysis (SID_GasAnalysis_NoGas, SID_GasAnalysis_NoGas);
-                      outp exited_GasAnalysis (SID_GasAnalysis_NoGas, SID_GasAnalysis_NoGas);
-                      outp enter_GasAnalysis (SID_GasAnalysis_NoGas, SID_GasAnalysis_Analysis);
-                      outp entered_GasAnalysis (SID_GasAnalysis_NoGas, SID_GasAnalysis_Analysis);
-                      Ret(False, fst (snd s), SID_GasAnalysis_NoGas)
+                      outp set_gs_Movement (snd (snd t)) ; 
+                      outp exit_Movement (SID_Movement_Waiting, SID_Movement_Waiting);
+                      outp exited_Movement (SID_Movement_Waiting, SID_Movement_Waiting);
+                      outp enter_Movement (SID_Movement_Waiting, SID_Movement_Analysis);
+                      outp entered_Movement (SID_Movement_Waiting, SID_Movement_Analysis);
+                      Ret(False, fst (snd s), SID_Movement_Waiting)
                     } \<box>
-                (exit_events_GasAnalysis (fst (snd s)) SID_GasAnalysis_NoGas 
-                   tids_GasAnalysis_NoGas Other_SIDs_to_NoGas_GasAnalysis)
+                (exit_events_Movement (fst (snd s)) SID_Movement_Waiting 
+                   tids_Movement_Waiting Other_SIDs_to_Waiting_Movement)
                 )
               )
             })
@@ -1332,84 +394,84 @@ definition State_GasAnalysis_NoGas where
 )
 "
 
-definition State_GasAnalysis_NoGas_R where
-"State_GasAnalysis_NoGas_R (idd::integer) = 
-   (discard_state (State_GasAnalysis_NoGas idd)) \<comment> \<open> discard state to match with skip on the right\<close>
-    \<parallel>\<^bsub> (int_int_GasAnalysis - GasAnalysis_NoGas_triggers) \<^esub> 
+definition State_Movement_Waiting_R where
+"State_Movement_Waiting_R (idd::integer) = 
+   (discard_state (State_Movement_Waiting idd)) \<comment> \<open> discard state to match with skip on the right\<close>
+    \<parallel>\<^bsub> (int_int_Movement - Movement_Waiting_triggers) \<^esub> 
    skip
 "
 
 paragraph \<open> Analysis \<close>
-definition CS_GasAnalysis_Analysis_sync where
-"CS_GasAnalysis_Analysis_sync = 
+definition CS_Movement_Analysis_sync where
+"CS_Movement_Analysis_sync = 
   set (
       \<comment> \<open> enter from x to y \<close>
-      (enumchans2 enter_exit_channels_GasAnalysis [SID_GasAnalysis_Analysis] SIDS_GasAnalysis_nodes)@
+      (enumchans2 enter_exit_channels_Movement [SID_Movement_Analysis] SIDS_Movement_nodes)@
       \<comment> \<open> enter from y to x \<close>
-      (enumchans2 enter_exit_channels_GasAnalysis SIDS_GasAnalysis_nodes [SID_GasAnalysis_Analysis])
+      (enumchans2 enter_exit_channels_Movement SIDS_Movement_nodes [SID_Movement_Analysis])
 )"
 
-definition GasAnalysis_Analysis_triggers where
-"GasAnalysis_Analysis_triggers = set (
-  (enumchan1 internal_GasAnalysis_C 
-    [TID_GasAnalysis_t3, TID_GasAnalysis_t4,
-     TID_GasAnalysis_t8, TID_GasAnalysis_t9a]) @
-  (enumchans3 [gas__GasAnalysis_C] 
-    [TID_GasAnalysis_t0, TID_GasAnalysis_t2] 
+definition Movement_Analysis_triggers where
+"Movement_Analysis_triggers = set (
+  (enumchan1 internal_Movement_C 
+    [TID_Movement_t3, TID_Movement_t4,
+     TID_Movement_t8, TID_Movement_t9a]) @
+  (enumchans3 [gas__Movement_C] 
+    [TID_Movement_t0, TID_Movement_t2] 
     [din, dout] 
     (lseq_gassensor_enum))
 )
 "
 
-definition tids_GasAnalysis_Analysis where
-" tids_GasAnalysis_Analysis = 
+definition tids_Movement_Analysis where
+" tids_Movement_Analysis = 
     (filter 
-        (\<lambda> s. s \<notin> {NULLTRANSITION__GasAnalysis, TID_GasAnalysis_t9a,
-          TID_GasAnalysis_t8, TID_GasAnalysis_t4, TID_GasAnalysis_t3, 
-          TID_GasAnalysis_t2, TID_GasAnalysis_t0}) 
-        ITIDS_GasAnalysis_list)"
+        (\<lambda> s. s \<notin> {NULLTRANSITION__Movement, TID_Movement_t9a,
+          TID_Movement_t8, TID_Movement_t4, TID_Movement_t3, 
+          TID_Movement_t2, TID_Movement_t0}) 
+        ITIDS_Movement_list)"
 
-abbreviation Other_SIDs_to_Analysis_GasAnalysis where
-"Other_SIDs_to_Analysis_GasAnalysis \<equiv> 
-  set [(s, SID_GasAnalysis_Analysis) . s \<leftarrow> (SIDS_GasAnalysis_no_Analysis)]"
+abbreviation Other_SIDs_to_Analysis_Movement where
+"Other_SIDs_to_Analysis_Movement \<equiv> 
+  set [(s, SID_Movement_Analysis) . s \<leftarrow> (SIDS_Movement_no_Analysis)]"
 
-definition State_GasAnalysis_Analysis where 
-"State_GasAnalysis_Analysis = 
+definition State_Movement_Analysis where 
+"State_Movement_Analysis = 
   loop (\<lambda> (id::integer).
-    do {sd \<leftarrow> inp_in enter_GasAnalysis Other_SIDs_to_Analysis_GasAnalysis ; 
+    do {sd \<leftarrow> inp_in enter_Movement Other_SIDs_to_Analysis_Movement ; 
         \<comment> \<open> State passed to next loop, including a condition initially True. \<close>
         ret \<leftarrow> Ret (True, id, fst sd) ; 
-        \<comment> \<open> State_GasAnalysis_Analysis_execute \<close>
+        \<comment> \<open> State_Movement_Analysis_execute \<close>
         (iterate 
            \<comment> \<open> condition \<close>
            (\<lambda> s. fst s) 
            \<comment> \<open> P \<close>
            (\<lambda> s.
             do {
-              gs \<leftarrow> inp_in get_gs_GasAnalysis (set (lseq_gassensor_enum));
-              outp set_st_GasAnalysis (Chemical_analysis gs);
-              outp entered_GasAnalysis (snd (snd s), SID_GasAnalysis_Analysis);
+              gs \<leftarrow> inp_in get_gs_Movement (set (lseq_gassensor_enum));
+              outp set_st_Movement (Chemical_analysis gs);
+              outp entered_Movement (snd (snd s), SID_Movement_Analysis);
               (do {skip ; stop} \<triangle>
                 (
-                \<comment> \<open> T_GasAnalysis_t3 \<close>
-                do {outp internal_GasAnalysis TID_GasAnalysis_t3 ;
-                    outp exit_GasAnalysis (SID_GasAnalysis_Analysis, SID_GasAnalysis_Analysis);
-                    outp exited_GasAnalysis (SID_GasAnalysis_Analysis, SID_GasAnalysis_Analysis);
-                    outp resume_GasAnalysis dout;
-                    outp enter_GasAnalysis (SID_GasAnalysis_Analysis, SID_GasAnalysis_NoGas);
-                    outp entered_GasAnalysis (SID_GasAnalysis_Analysis, SID_GasAnalysis_NoGas);
-                    Ret(False, fst (snd s), SID_GasAnalysis_Analysis)
+                \<comment> \<open> T_Movement_t3 \<close>
+                do {outp internal_Movement TID_Movement_t3 ;
+                    outp exit_Movement (SID_Movement_Analysis, SID_Movement_Analysis);
+                    outp exited_Movement (SID_Movement_Analysis, SID_Movement_Analysis);
+                    outp resume_Movement dout;
+                    outp enter_Movement (SID_Movement_Analysis, SID_Movement_Waiting);
+                    outp entered_Movement (SID_Movement_Analysis, SID_Movement_Waiting);
+                    Ret(False, fst (snd s), SID_Movement_Analysis)
                     } \<box>
-                \<comment> \<open> T_GasAnalysis_t4 \<close>
-                do {outp internal_GasAnalysis TID_GasAnalysis_t4 ;
-                    outp exit_GasAnalysis (SID_GasAnalysis_Analysis, SID_GasAnalysis_Analysis);
-                    outp exited_GasAnalysis (SID_GasAnalysis_Analysis, SID_GasAnalysis_Analysis);
-                    outp enter_GasAnalysis (SID_GasAnalysis_Analysis, SID_GasAnalysis_GasDetected);
-                    outp entered_GasAnalysis (SID_GasAnalysis_Analysis, SID_GasAnalysis_GasDetected);
-                    Ret(False, fst (snd s), SID_GasAnalysis_Analysis)
+                \<comment> \<open> T_Movement_t4 \<close>
+                do {outp internal_Movement TID_Movement_t4 ;
+                    outp exit_Movement (SID_Movement_Analysis, SID_Movement_Analysis);
+                    outp exited_Movement (SID_Movement_Analysis, SID_Movement_Analysis);
+                    outp enter_Movement (SID_Movement_Analysis, SID_Movement_GasDetected);
+                    outp entered_Movement (SID_Movement_Analysis, SID_Movement_GasDetected);
+                    Ret(False, fst (snd s), SID_Movement_Analysis)
                     } \<box>
-                (exit_events_GasAnalysis (fst (snd s)) SID_GasAnalysis_Analysis 
-                   tids_GasAnalysis_Analysis Other_SIDs_to_Analysis_GasAnalysis)
+                (exit_events_Movement (fst (snd s)) SID_Movement_Analysis 
+                   tids_Movement_Analysis Other_SIDs_to_Analysis_Movement)
                 )
               )
             })
@@ -1421,90 +483,90 @@ definition State_GasAnalysis_Analysis where
 )
 "
 
-definition State_GasAnalysis_Analysis_R where
-"State_GasAnalysis_Analysis_R (idd::integer) = 
-   (discard_state (State_GasAnalysis_Analysis idd)) \<comment> \<open> discard state to match with skip on the right\<close>
-    \<parallel>\<^bsub> (int_int_GasAnalysis - GasAnalysis_Analysis_triggers) \<^esub> 
+definition State_Movement_Analysis_R where
+"State_Movement_Analysis_R (idd::integer) = 
+   (discard_state (State_Movement_Analysis idd)) \<comment> \<open> discard state to match with skip on the right\<close>
+    \<parallel>\<^bsub> (int_int_Movement - Movement_Analysis_triggers) \<^esub> 
    skip
 "
 
 paragraph \<open> GasDetected \<close>
-definition CS_GasAnalysis_GasDetected_sync where
-"CS_GasAnalysis_GasDetected_sync = 
+definition CS_Movement_GasDetected_sync where
+"CS_Movement_GasDetected_sync = 
   set (
       \<comment> \<open> enter from x to y \<close>
-      (enumchans2 enter_exit_channels_GasAnalysis [SID_GasAnalysis_GasDetected] SIDS_GasAnalysis_nodes)@
+      (enumchans2 enter_exit_channels_Movement [SID_Movement_GasDetected] SIDS_Movement_nodes)@
       \<comment> \<open> enter from y to x \<close>
-      (enumchans2 enter_exit_channels_GasAnalysis SIDS_GasAnalysis_nodes [SID_GasAnalysis_GasDetected])
+      (enumchans2 enter_exit_channels_Movement SIDS_Movement_nodes [SID_Movement_GasDetected])
 )"
 
-definition GasAnalysis_GasDetected_triggers where
-"GasAnalysis_GasDetected_triggers = set (
-  (enumchan1 internal_GasAnalysis_C 
-    [TID_GasAnalysis_t3, TID_GasAnalysis_t4,
-     TID_GasAnalysis_t8, TID_GasAnalysis_t9a]) @
-  (enumchans3 [gas__GasAnalysis_C] 
-    [TID_GasAnalysis_t0, TID_GasAnalysis_t2] 
+definition Movement_GasDetected_triggers where
+"Movement_GasDetected_triggers = set (
+  (enumchan1 internal_Movement_C 
+    [TID_Movement_t3, TID_Movement_t4,
+     TID_Movement_t8, TID_Movement_t9a]) @
+  (enumchans3 [gas__Movement_C] 
+    [TID_Movement_t0, TID_Movement_t2] 
     [din, dout] 
     (lseq_gassensor_enum))
 )
 "
 
-definition tids_GasAnalysis_GasDetected where
-" tids_GasAnalysis_GasDetected = 
+definition tids_Movement_GasDetected where
+" tids_Movement_GasDetected = 
     (filter 
-        (\<lambda> s. s \<notin> {NULLTRANSITION__GasAnalysis, TID_GasAnalysis_t9a,
-          TID_GasAnalysis_t8, TID_GasAnalysis_t4, TID_GasAnalysis_t3, 
-          TID_GasAnalysis_t2, TID_GasAnalysis_t0}) 
-        ITIDS_GasAnalysis_list)"
+        (\<lambda> s. s \<notin> {NULLTRANSITION__Movement, TID_Movement_t9a,
+          TID_Movement_t8, TID_Movement_t4, TID_Movement_t3, 
+          TID_Movement_t2, TID_Movement_t0}) 
+        ITIDS_Movement_list)"
 
-abbreviation Other_SIDs_to_GasDetected_GasAnalysis where
-"Other_SIDs_to_GasDetected_GasAnalysis \<equiv>
-  set [(s, SID_GasAnalysis_GasDetected) . s \<leftarrow> (SIDS_GasAnalysis_no_GasDetected)]"
+abbreviation Other_SIDs_to_GasDetected_Movement where
+"Other_SIDs_to_GasDetected_Movement \<equiv>
+  set [(s, SID_Movement_GasDetected) . s \<leftarrow> (SIDS_Movement_no_GasDetected)]"
 
-definition State_GasAnalysis_GasDetected where 
-"State_GasAnalysis_GasDetected = 
+definition State_Movement_GasDetected where 
+"State_Movement_GasDetected = 
   loop (\<lambda> (id::integer).
-    do {sd \<leftarrow> inp_in enter_GasAnalysis Other_SIDs_to_GasDetected_GasAnalysis ; 
+    do {sd \<leftarrow> inp_in enter_Movement Other_SIDs_to_GasDetected_Movement ; 
         \<comment> \<open> State passed to next loop, including a condition initially True. \<close>
         ret \<leftarrow> Ret (True, id, fst sd) ; 
-        \<comment> \<open> State_GasAnalysis_GasDetected_execute \<close>
+        \<comment> \<open> State_Movement_GasDetected_execute \<close>
         (iterate 
            \<comment> \<open> condition \<close>
            (\<lambda> s. fst s) 
            \<comment> \<open> P \<close>
            (\<lambda> s.
             do {
-              gs \<leftarrow> inp_in get_gs_GasAnalysis (set (lseq_gassensor_enum));
+              gs \<leftarrow> inp_in get_gs_Movement (set (lseq_gassensor_enum));
               guard (pre_Chemical_intensity(gs));
-              outp set_i_GasAnalysis (Chemical_intensity gs);
-              outp entered_GasAnalysis (snd (snd s), SID_GasAnalysis_GasDetected);
+              outp set_i_Movement (Chemical_intensity gs);
+              outp entered_Movement (snd (snd s), SID_Movement_GasDetected);
               (do {skip ; stop} \<triangle>
                 (
-                \<comment> \<open> T_GasAnalysis_t8 \<close>
-                do {outp internal_GasAnalysis TID_GasAnalysis_t8 ;
-                    outp exit_GasAnalysis (SID_GasAnalysis_GasDetected, SID_GasAnalysis_GasDetected);
-                    outp exited_GasAnalysis (SID_GasAnalysis_GasDetected, SID_GasAnalysis_GasDetected);
-                    outp stop_GasAnalysis dout;
-                    outp enter_GasAnalysis (SID_GasAnalysis_GasDetected, SID_GasAnalysis_j1);
-                    outp entered_GasAnalysis (SID_GasAnalysis_GasDetected, SID_GasAnalysis_j1);
-                    Ret(False, fst (snd s), SID_GasAnalysis_GasDetected)
+                \<comment> \<open> T_Movement_t8 \<close>
+                do {outp internal_Movement TID_Movement_t8 ;
+                    outp exit_Movement (SID_Movement_GasDetected, SID_Movement_GasDetected);
+                    outp exited_Movement (SID_Movement_GasDetected, SID_Movement_GasDetected);
+                    outp stop_Movement dout;
+                    outp enter_Movement (SID_Movement_GasDetected, SID_Movement_j1);
+                    outp entered_Movement (SID_Movement_GasDetected, SID_Movement_j1);
+                    Ret(False, fst (snd s), SID_Movement_GasDetected)
                     } \<box>
-                 \<comment> \<open> T_GasAnalysis_t9a \<close>
-                do {outp internal_GasAnalysis TID_GasAnalysis_t9a ;
-                    outp exit_GasAnalysis (SID_GasAnalysis_GasDetected, SID_GasAnalysis_GasDetected);
-                    outp exited_GasAnalysis (SID_GasAnalysis_GasDetected, SID_GasAnalysis_GasDetected);
-                    gs \<leftarrow> inp_in get_gs_GasAnalysis (set (lseq_gassensor_enum));
+                 \<comment> \<open> T_Movement_t9a \<close>
+                do {outp internal_Movement TID_Movement_t9a ;
+                    outp exit_Movement (SID_Movement_GasDetected, SID_Movement_GasDetected);
+                    outp exited_Movement (SID_Movement_GasDetected, SID_Movement_GasDetected);
+                    gs \<leftarrow> inp_in get_gs_Movement (set (lseq_gassensor_enum));
                     guard (pre_Chemical_location(gs));
-                    outp set_a_GasAnalysis (Chemical_location gs);
-                    a \<leftarrow> inp_in get_a_GasAnalysis Chemical_Angle_set;
-                    outp turn_GasAnalysis (dout, a);
-                    outp enter_GasAnalysis (SID_GasAnalysis_GasDetected, SID_GasAnalysis_Reading);
-                    outp entered_GasAnalysis (SID_GasAnalysis_GasDetected, SID_GasAnalysis_Reading);
-                    Ret(False, fst (snd s), SID_GasAnalysis_GasDetected)
+                    outp set_a_Movement (Chemical_location gs);
+                    a \<leftarrow> inp_in get_a_Movement Chemical_Angle_set;
+                    outp turn_Movement (dout, a);
+                    outp enter_Movement (SID_Movement_GasDetected, SID_Movement_Reading);
+                    outp entered_Movement (SID_Movement_GasDetected, SID_Movement_Reading);
+                    Ret(False, fst (snd s), SID_Movement_GasDetected)
                     } \<box>
-                (exit_events_GasAnalysis (fst (snd s)) SID_GasAnalysis_GasDetected 
-                   tids_GasAnalysis_GasDetected Other_SIDs_to_GasDetected_GasAnalysis)
+                (exit_events_Movement (fst (snd s)) SID_Movement_GasDetected 
+                   tids_Movement_GasDetected Other_SIDs_to_GasDetected_Movement)
                 )
               )
             })
@@ -1516,118 +578,118 @@ definition State_GasAnalysis_GasDetected where
 )
 "
 
-definition State_GasAnalysis_GasDetected_R where
-"State_GasAnalysis_GasDetected_R (idd::integer) = 
-   (discard_state (State_GasAnalysis_GasDetected idd)) \<comment> \<open> discard state to match with skip on the right\<close>
-    \<parallel>\<^bsub> (int_int_GasAnalysis - GasAnalysis_GasDetected_triggers) \<^esub> 
+definition State_Movement_GasDetected_R where
+"State_Movement_GasDetected_R (idd::integer) = 
+   (discard_state (State_Movement_GasDetected idd)) \<comment> \<open> discard state to match with skip on the right\<close>
+    \<parallel>\<^bsub> (int_int_Movement - Movement_GasDetected_triggers) \<^esub> 
    skip
 "
 
 paragraph \<open> Final \<close>
-definition CS_GasAnalysis_j1_sync where
-"CS_GasAnalysis_j1_sync = 
+definition CS_Movement_j1_sync where
+"CS_Movement_j1_sync = 
   set (
       \<comment> \<open> enter from x to y \<close>
-      (enumchans2 enter_exit_channels_GasAnalysis [SID_GasAnalysis_j1] SIDS_GasAnalysis_nodes)@
+      (enumchans2 enter_exit_channels_Movement [SID_Movement_j1] SIDS_Movement_nodes)@
       \<comment> \<open> enter from y to x \<close>
-      (enumchans2 enter_exit_channels_GasAnalysis SIDS_GasAnalysis_nodes [SID_GasAnalysis_j1])
+      (enumchans2 enter_exit_channels_Movement SIDS_Movement_nodes [SID_Movement_j1])
 )"
 
-definition GasAnalysis_j1_triggers where
-"GasAnalysis_j1_triggers = set ([])
+definition Movement_j1_triggers where
+"Movement_j1_triggers = set ([])
 "
 
-definition tids_GasAnalysis_j1 where
-" tids_GasAnalysis_j1 = 
+definition tids_Movement_j1 where
+" tids_Movement_j1 = 
     (filter 
-        (\<lambda> s. s \<notin> {NULLTRANSITION__GasAnalysis, TID_GasAnalysis_t9a,
-          TID_GasAnalysis_t8, TID_GasAnalysis_t4, TID_GasAnalysis_t3, 
-          TID_GasAnalysis_t2, TID_GasAnalysis_t0}) 
-        ITIDS_GasAnalysis_list)"
+        (\<lambda> s. s \<notin> {NULLTRANSITION__Movement, TID_Movement_t9a,
+          TID_Movement_t8, TID_Movement_t4, TID_Movement_t3, 
+          TID_Movement_t2, TID_Movement_t0}) 
+        ITIDS_Movement_list)"
 
-abbreviation Other_SIDs_to_j1_GasAnalysis where
-"Other_SIDs_to_j1_GasAnalysis \<equiv>
-  set [(s, SID_GasAnalysis_j1) . s \<leftarrow> (SIDS_GasAnalysis_no_j1)]"
+abbreviation Other_SIDs_to_j1_Movement where
+"Other_SIDs_to_j1_Movement \<equiv>
+  set [(s, SID_Movement_j1) . s \<leftarrow> (SIDS_Movement_no_j1)]"
 
-definition State_GasAnalysis_j1 where 
-"State_GasAnalysis_j1 = 
+definition State_Movement_j1 where 
+"State_Movement_j1 = 
   loop (\<lambda> (id::integer).
-    do {sd \<leftarrow> inp_in enter_GasAnalysis Other_SIDs_to_j1_GasAnalysis ; 
-        outp terminate_GasAnalysis ();
+    do {sd \<leftarrow> inp_in enter_Movement Other_SIDs_to_j1_Movement ; 
+        outp terminate_Movement ();
         Ret (id)
     }
 )
 "
 
-definition State_GasAnalysis_j1_R where
-"State_GasAnalysis_j1_R (idd::integer) = 
-   (discard_state (State_GasAnalysis_j1 idd)) \<comment> \<open> discard state to match with skip on the right\<close>
-    \<parallel>\<^bsub> (int_int_GasAnalysis - GasAnalysis_j1_triggers) \<^esub> 
+definition State_Movement_j1_R where
+"State_Movement_j1_R (idd::integer) = 
+   (discard_state (State_Movement_j1 idd)) \<comment> \<open> discard state to match with skip on the right\<close>
+    \<parallel>\<^bsub> (int_int_Movement - Movement_j1_triggers) \<^esub> 
    skip
 "
 
 paragraph \<open> Reading \<close>
-definition CS_GasAnalysis_Reading_sync where
-"CS_GasAnalysis_Reading_sync = 
+definition CS_Movement_Reading_sync where
+"CS_Movement_Reading_sync = 
   set (
       \<comment> \<open> enter from x to y \<close>
-      (enumchans2 enter_exit_channels_GasAnalysis [SID_GasAnalysis_Reading] SIDS_GasAnalysis_nodes)@
+      (enumchans2 enter_exit_channels_Movement [SID_Movement_Reading] SIDS_Movement_nodes)@
       \<comment> \<open> enter from y to x \<close>
-      (enumchans2 enter_exit_channels_GasAnalysis SIDS_GasAnalysis_nodes [SID_GasAnalysis_Reading])
+      (enumchans2 enter_exit_channels_Movement SIDS_Movement_nodes [SID_Movement_Reading])
 )"
 
-definition GasAnalysis_Reading_triggers where
-"GasAnalysis_Reading_triggers = set (
-  (enumchan1 internal_GasAnalysis_C 
-    [TID_GasAnalysis_t3, TID_GasAnalysis_t4,
-     TID_GasAnalysis_t8, TID_GasAnalysis_t9a]) @
-  (enumchans3 [gas__GasAnalysis_C] 
-    [TID_GasAnalysis_t0, TID_GasAnalysis_t2] 
+definition Movement_Reading_triggers where
+"Movement_Reading_triggers = set (
+  (enumchan1 internal_Movement_C 
+    [TID_Movement_t3, TID_Movement_t4,
+     TID_Movement_t8, TID_Movement_t9a]) @
+  (enumchans3 [gas__Movement_C] 
+    [TID_Movement_t0, TID_Movement_t2] 
     [din, dout] 
     (lseq_gassensor_enum))
 )
 "
 
-definition tids_GasAnalysis_Reading where
-" tids_GasAnalysis_Reading = 
+definition tids_Movement_Reading where
+" tids_Movement_Reading = 
     (filter 
-        (\<lambda> s. s \<notin> {NULLTRANSITION__GasAnalysis, TID_GasAnalysis_t9a,
-          TID_GasAnalysis_t8, TID_GasAnalysis_t4, TID_GasAnalysis_t3, 
-          TID_GasAnalysis_t2, TID_GasAnalysis_t0}) 
-        ITIDS_GasAnalysis_list)"
+        (\<lambda> s. s \<notin> {NULLTRANSITION__Movement, TID_Movement_t9a,
+          TID_Movement_t8, TID_Movement_t4, TID_Movement_t3, 
+          TID_Movement_t2, TID_Movement_t0}) 
+        ITIDS_Movement_list)"
 
-abbreviation Other_SIDs_to_Reading_GasAnalysis where
-"Other_SIDs_to_Reading_GasAnalysis \<equiv>
-  set [(s, SID_GasAnalysis_Reading) . s \<leftarrow> (SIDS_GasAnalysis_no_Reading)]"
+abbreviation Other_SIDs_to_Reading_Movement where
+"Other_SIDs_to_Reading_Movement \<equiv>
+  set [(s, SID_Movement_Reading) . s \<leftarrow> (SIDS_Movement_no_Reading)]"
 
-definition State_GasAnalysis_Reading where 
-"State_GasAnalysis_Reading = 
+definition State_Movement_Reading where 
+"State_Movement_Reading = 
   loop (\<lambda> (id::integer).
-    do {sd \<leftarrow> inp_in enter_GasAnalysis Other_SIDs_to_Reading_GasAnalysis ; 
+    do {sd \<leftarrow> inp_in enter_Movement Other_SIDs_to_Reading_Movement ; 
         \<comment> \<open> State passed to next loop, including a condition initially True. \<close>
         ret \<leftarrow> Ret (True, id, fst sd) ; 
-        \<comment> \<open> State_GasAnalysis_Reading_execute \<close>
+        \<comment> \<open> State_Movement_Reading_execute \<close>
         (iterate 
            \<comment> \<open> condition \<close>
            (\<lambda> s. fst s) 
            \<comment> \<open> P \<close>
            (\<lambda> s.
             do {
-              outp entered_GasAnalysis (snd (snd s), SID_GasAnalysis_Reading);
+              outp entered_Movement (snd (snd s), SID_Movement_Reading);
               (do {skip ; stop} \<triangle>
                 (
-                \<comment> \<open> T_GasAnalysis_t0 \<close>
-                do {gs \<leftarrow> inp_in gas__GasAnalysis (set [(TID_GasAnalysis_t0, din, x). 
+                \<comment> \<open> T_Movement_t0 \<close>
+                do {gs \<leftarrow> inp_in gas__Movement (set [(TID_Movement_t0, din, x). 
                         x \<leftarrow> (lseq_gassensor_enum)]) ;
-                    outp set_gs_GasAnalysis (snd (snd gs));
-                    outp exit_GasAnalysis (SID_GasAnalysis_Reading, SID_GasAnalysis_Reading);
-                    outp exited_GasAnalysis (SID_GasAnalysis_Reading, SID_GasAnalysis_Reading);
-                    outp enter_GasAnalysis (SID_GasAnalysis_Reading, SID_GasAnalysis_Analysis);
-                    outp entered_GasAnalysis (SID_GasAnalysis_Reading, SID_GasAnalysis_Analysis);
-                    Ret(False, fst (snd s), SID_GasAnalysis_Reading)
+                    outp set_gs_Movement (snd (snd gs));
+                    outp exit_Movement (SID_Movement_Reading, SID_Movement_Reading);
+                    outp exited_Movement (SID_Movement_Reading, SID_Movement_Reading);
+                    outp enter_Movement (SID_Movement_Reading, SID_Movement_Analysis);
+                    outp entered_Movement (SID_Movement_Reading, SID_Movement_Analysis);
+                    Ret(False, fst (snd s), SID_Movement_Reading)
                     } \<box>
-                (exit_events_GasAnalysis (fst (snd s)) SID_GasAnalysis_Reading 
-                   tids_GasAnalysis_Reading Other_SIDs_to_Reading_GasAnalysis)
+                (exit_events_Movement (fst (snd s)) SID_Movement_Reading 
+                   tids_Movement_Reading Other_SIDs_to_Reading_Movement)
                 )
               )
             })
@@ -1639,154 +701,154 @@ definition State_GasAnalysis_Reading where
 )
 "
 
-definition State_GasAnalysis_Reading_R where
-"State_GasAnalysis_Reading_R (idd::integer) = 
-   (discard_state (State_GasAnalysis_Reading idd)) \<comment> \<open> discard state to match with skip on the right\<close>
-    \<parallel>\<^bsub> (int_int_GasAnalysis - GasAnalysis_Reading_triggers) \<^esub> 
+definition State_Movement_Reading_R where
+"State_Movement_Reading_R (idd::integer) = 
+   (discard_state (State_Movement_Reading idd)) \<comment> \<open> discard state to match with skip on the right\<close>
+    \<parallel>\<^bsub> (int_int_Movement - Movement_Reading_triggers) \<^esub> 
    skip
 "
 
 subsubsection \<open> State machine \<close>
-definition flow_events_GasAnalysis_stm_to_nodes where
-"flow_events_GasAnalysis_stm_to_nodes = (
- let nodes = [SID_GasAnalysis_NoGas,SID_GasAnalysis_Analysis,SID_GasAnalysis_GasDetected,
-              SID_GasAnalysis_j1,SID_GasAnalysis_Reading]
+definition flow_events_Movement_stm_to_nodes where
+"flow_events_Movement_stm_to_nodes = (
+ let nodes = [SID_Movement_Waiting,SID_Movement_Analysis,SID_Movement_GasDetected,
+              SID_Movement_j1,SID_Movement_Reading]
  in set (
-      enumchans2 [enter_GasAnalysis_C, entered_GasAnalysis_C,exit_GasAnalysis_C,exited_GasAnalysis_C] 
-          (filter (\<lambda> s. s \<notin> set nodes) SIDS_GasAnalysis_list) nodes
+      enumchans2 [enter_Movement_C, entered_Movement_C,exit_Movement_C,exited_Movement_C] 
+          (filter (\<lambda> s. s \<notin> set nodes) SIDS_Movement_list) nodes
   )
 )"
 
-definition STM_GasAnalysis where
-"STM_GasAnalysis (idd::integer) = 
-   (I_GasAnalysis_i1(idd))
-    \<parallel>\<^bsub> flow_events_GasAnalysis_stm_to_nodes \<^esub> 
-   (State_GasAnalysis_NoGas_R(idd)
-      \<parallel>\<^bsub> CS_GasAnalysis_Analysis_sync \<inter> (CS_GasAnalysis_Analysis_sync \<union> 
-          (CS_GasAnalysis_GasDetected_sync \<union> (CS_GasAnalysis_j1_sync \<union> CS_GasAnalysis_Reading_sync))) \<^esub>
-      (State_GasAnalysis_Analysis_R(idd)
-        \<parallel>\<^bsub> CS_GasAnalysis_Analysis_sync \<inter> (CS_GasAnalysis_GasDetected_sync \<union> 
-            (CS_GasAnalysis_j1_sync \<union> CS_GasAnalysis_Reading_sync)) \<^esub> 
-        ( State_GasAnalysis_GasDetected_R(idd)
-          \<parallel>\<^bsub> CS_GasAnalysis_GasDetected_sync \<inter> (CS_GasAnalysis_j1_sync \<union> CS_GasAnalysis_Reading_sync) \<^esub> 
-          (State_GasAnalysis_j1_R(idd)  
-            \<parallel>\<^bsub> CS_GasAnalysis_j1_sync \<inter> CS_GasAnalysis_Reading_sync \<^esub> 
-          State_GasAnalysis_Reading_R(idd))
+definition STM_Movement where
+"STM_Movement (idd::integer) = 
+   (I_Movement_i1(idd))
+    \<parallel>\<^bsub> flow_events_Movement_stm_to_nodes \<^esub> 
+   (State_Movement_Waiting_R(idd)
+      \<parallel>\<^bsub> CS_Movement_Analysis_sync \<inter> (CS_Movement_Analysis_sync \<union> 
+          (CS_Movement_GasDetected_sync \<union> (CS_Movement_j1_sync \<union> CS_Movement_Reading_sync))) \<^esub>
+      (State_Movement_Analysis_R(idd)
+        \<parallel>\<^bsub> CS_Movement_Analysis_sync \<inter> (CS_Movement_GasDetected_sync \<union> 
+            (CS_Movement_j1_sync \<union> CS_Movement_Reading_sync)) \<^esub> 
+        ( State_Movement_GasDetected_R(idd)
+          \<parallel>\<^bsub> CS_Movement_GasDetected_sync \<inter> (CS_Movement_j1_sync \<union> CS_Movement_Reading_sync) \<^esub> 
+          (State_Movement_j1_R(idd)  
+            \<parallel>\<^bsub> CS_Movement_j1_sync \<inter> CS_Movement_Reading_sync \<^esub> 
+          State_Movement_Reading_R(idd))
         )
       )
    )
 "
 
-definition GasAnalysis_opt_0_internal_set where
-"GasAnalysis_opt_0_internal_set = 
-  set (([internal_GasAnalysis_C TID_GasAnalysis_t1]) @ 
-       (enumchans3 [gas__GasAnalysis_C] 
-          [TID_GasAnalysis_t0, TID_GasAnalysis_t2] 
+definition Movement_opt_0_internal_set where
+"Movement_opt_0_internal_set = 
+  set (([internal_Movement_C TID_Movement_t1]) @ 
+       (enumchans3 [gas__Movement_C] 
+          [TID_Movement_t0, TID_Movement_t2] 
           [din, dout] 
           (lseq_gassensor_enum))
 )"
 
-definition GasAnalysis_opt_1_internal_set where
-"GasAnalysis_opt_1_internal_set = 
-  set ((enumchans1 [internal_GasAnalysis_C] [TID_GasAnalysis_t4, TID_GasAnalysis_t3]) @
-       (enumchans1 [set_st_GasAnalysis_C] Chemical_Status_list)
+definition Movement_opt_1_internal_set where
+"Movement_opt_1_internal_set = 
+  set ((enumchans1 [internal_Movement_C] [TID_Movement_t4, TID_Movement_t3]) @
+       (enumchans1 [set_st_Movement_C] Chemical_Status_list)
 )"
 
-definition GasAnalysis_opt_2_internal_set where
-"GasAnalysis_opt_2_internal_set = 
-  set ((enumchans1 [internal_GasAnalysis_C] [TID_GasAnalysis_t8, TID_GasAnalysis_t9a])
+definition Movement_opt_2_internal_set where
+"Movement_opt_2_internal_set = 
+  set ((enumchans1 [internal_Movement_C] [TID_Movement_t8, TID_Movement_t9a])
 )"
 
-definition MemorySTM_opt_GasAnalysis where
-"MemorySTM_opt_GasAnalysis (idd::integer) = 
+definition MemorySTM_opt_Movement where
+"MemorySTM_opt_Movement (idd::integer) = 
   (par_hide
-    (discard_state (GasAnalysis_Memory_opt_i (Chemical_IntensityC (0::2))))
-    GasAnalysis_i_events
+    (discard_state (Movement_Memory_opt_i (Chemical_IntensityC (0::2))))
+    Movement_i_events
     (par_hide 
       (par_hide
-        (discard_state (GasAnalysis_Memory_opt_st (Chemical_Status_noGas)))
-        GasAnalysis_st_events
+        (discard_state (Movement_Memory_opt_st (Chemical_Status_noGas)))
+        Movement_st_events
         (hide 
           (
             (hide
               (
                 (par_hide
-                  (discard_state (GasAnalysis_Memory_opt_gs (bmake TYPE(2) [])))
-                  GasAnalysis_gs_events
+                  (discard_state (Movement_Memory_opt_gs (bmake TYPE(2) [])))
+                  Movement_gs_events
                   (par_hide 
-                    (discard_state (GasAnalysis_Memory_opt_a Chemical_Angle_Left)) 
-                    GasAnalysis_a_events 
-                    (STM_GasAnalysis idd)
+                    (discard_state (Movement_Memory_opt_a Chemical_Angle_Left)) 
+                    Movement_a_events 
+                    (STM_Movement idd)
                   )
                 )
-                \<parallel>\<^bsub> GasAnalysis_opt_0_internal_set \<^esub>
-                (discard_state (GasAnalysis_MemoryTransitions_opt_0 idd))
+                \<parallel>\<^bsub> Movement_opt_0_internal_set \<^esub>
+                (discard_state (Movement_MemoryTransitions_opt_0 idd))
               )
-              ({internal_GasAnalysis_C TID_GasAnalysis_t1})
+              ({internal_Movement_C TID_Movement_t1})
             )
-            \<parallel>\<^bsub> GasAnalysis_opt_1_internal_set \<^esub> 
-            (discard_state (GasAnalysis_MemoryTransitions_opt_1 idd))
+            \<parallel>\<^bsub> Movement_opt_1_internal_set \<^esub> 
+            (discard_state (Movement_MemoryTransitions_opt_1 idd))
           )
-          (set (enumchans1 [internal_GasAnalysis_C] [TID_GasAnalysis_t4, TID_GasAnalysis_t3]))
+          (set (enumchans1 [internal_Movement_C] [TID_Movement_t4, TID_Movement_t3]))
         )
       )
-      GasAnalysis_opt_2_internal_set
-      (discard_state (GasAnalysis_MemoryTransitions_opt_2 idd))
+      Movement_opt_2_internal_set
+      (discard_state (Movement_MemoryTransitions_opt_2 idd))
     )
   )   
 "
 
-definition rename_GasAnalysis_events where
-"rename_GasAnalysis_events = 
+definition rename_Movement_events where
+"rename_Movement_events = 
   concat (
-    (enumchan2 (forget_first2 gas__GasAnalysis_C gas_GasAnalysis_C TIDS_GasAnalysis_list) 
+    (enumchan2 (forget_first2 gas__Movement_C gas_Movement_C TIDS_Movement_list) 
             InOut_list lseq_gassensor_enum) @
-    (enumchan2 (forget_first2 turn__GasAnalysis_C turn_GasAnalysis_C TIDS_GasAnalysis_list) 
+    (enumchan2 (forget_first2 turn__Movement_C turn_Movement_C TIDS_Movement_list) 
             InOut_list Chemical_Angle_list) @
-    (enumchan1 (forget_first resume__GasAnalysis_C resume_GasAnalysis_C TIDS_GasAnalysis_list) 
+    (enumchan1 (forget_first resume__Movement_C resume_Movement_C TIDS_Movement_list) 
             InOut_list) @
-    (enumchan1 (forget_first stop__GasAnalysis_C stop_GasAnalysis_C TIDS_GasAnalysis_list) 
+    (enumchan1 (forget_first stop__Movement_C stop_Movement_C TIDS_Movement_list) 
             InOut_list)
   )
 "
 
-term "\<lbrace>resume__GasAnalysis (t, x) \<mapsto> resume_GasAnalysis x | x. x \<in> InOut_set\<rbrace>"
-term "\<lbrace>terminate_GasAnalysis () \<mapsto> terminate_GasAnalysis () | _. True\<rbrace>"
+term "\<lbrace>resume__Movement (t, x) \<mapsto> resume_Movement x | x. x \<in> InOut_set\<rbrace>"
+term "\<lbrace>terminate_Movement () \<mapsto> terminate_Movement () | _. True\<rbrace>"
 
-definition rename_GasAnalysis_events_others where
-"rename_GasAnalysis_events_others = 
-  (enumchanp1 terminate_GasAnalysis_C [()]) @
-  (enumchansp1 [get_i_GasAnalysis_C, set_i_GasAnalysis_C] Chemical_Intensity2_list) @
-  (enumchansp1 [get_a_GasAnalysis_C, set_a_GasAnalysis_C] Chemical_Angle_list) @
-  (enumchansp1 [get_st_GasAnalysis_C, set_st_GasAnalysis_C] Chemical_Status_list) @
-  (enumchansp1 [get_gs_GasAnalysis_C, set_gs_GasAnalysis_C] lseq_gassensor_enum) @
-  (enumchansp2 [gas_GasAnalysis_C] InOut_list lseq_gassensor_enum) @
-  (enumchansp2 [turn_GasAnalysis_C] InOut_list Chemical_Angle_list) @
-  (enumchansp1 [resume_GasAnalysis_C, stop_GasAnalysis_C] InOut_list) @
-  (enumchansp2 [enter_GasAnalysis_C, entered_GasAnalysis_C, exit_GasAnalysis_C, exited_GasAnalysis_C] 
-    SIDS_GasAnalysis_list SIDS_GasAnalysis_list) @
-  (enumchansp1 [internal_GasAnalysis_C] TIDS_GasAnalysis_list)
+definition rename_Movement_events_others where
+"rename_Movement_events_others = 
+  (enumchanp1 terminate_Movement_C [()]) @
+  (enumchansp1 [get_i_Movement_C, set_i_Movement_C] Chemical_Intensity2_list) @
+  (enumchansp1 [get_a_Movement_C, set_a_Movement_C] Chemical_Angle_list) @
+  (enumchansp1 [get_st_Movement_C, set_st_Movement_C] Chemical_Status_list) @
+  (enumchansp1 [get_gs_Movement_C, set_gs_Movement_C] lseq_gassensor_enum) @
+  (enumchansp2 [gas_Movement_C] InOut_list lseq_gassensor_enum) @
+  (enumchansp2 [turn_Movement_C] InOut_list Chemical_Angle_list) @
+  (enumchansp1 [resume_Movement_C, stop_Movement_C] InOut_list) @
+  (enumchansp2 [enter_Movement_C, entered_Movement_C, exit_Movement_C, exited_Movement_C] 
+    SIDS_Movement_list SIDS_Movement_list) @
+  (enumchansp1 [internal_Movement_C] TIDS_Movement_list)
 "
 
-definition rename_MemorySTM_opt_GasAnalysis where
-"rename_MemorySTM_opt_GasAnalysis idd = 
-  rename (set (rename_GasAnalysis_events @ rename_GasAnalysis_events_others)) 
-    (MemorySTM_opt_GasAnalysis idd)
+definition rename_MemorySTM_opt_Movement where
+"rename_MemorySTM_opt_Movement idd = 
+  rename (set (rename_Movement_events @ rename_Movement_events_others)) 
+    (MemorySTM_opt_Movement idd)
 "
 
-definition AUX_opt_GasAnalysis where
-"AUX_opt_GasAnalysis (idd::integer) = 
+definition AUX_opt_Movement where
+"AUX_opt_Movement (idd::integer) = 
   (hide 
     ( 
-      (rename_MemorySTM_opt_GasAnalysis idd) \<lbrakk> set [terminate_GasAnalysis_C ()] \<Zrres> skip
+      (rename_MemorySTM_opt_Movement idd) \<lbrakk> set [terminate_Movement_C ()] \<Zrres> skip
     )
-    GasAnalysis_MachineInternalEvents
+    Movement_MachineInternalEvents
   )
 "
 
-definition D__GasAnalysis where
-"D__GasAnalysis (idd::integer) = 
-  hide (AUX_opt_GasAnalysis idd) internal_events_GasAnalysis
+definition D__Movement where
+"D__Movement (idd::integer) = 
+  hide (AUX_opt_Movement idd) internal_events_Movement
 "
 
 subsection \<open> MainController \<close>
@@ -1803,44 +865,44 @@ definition Memory_MainCtrl where
 
 subsubsection \<open> Controller \<close>
 
-definition rename_MainCtrl_GasAnalysis_events where
-"rename_MainCtrl_GasAnalysis_events = 
-  (enumchanp2_1 (terminate_GasAnalysis_C,terminate_MainCtrl_C) [()]) @
-  (enumchansp2_2 [(gas_GasAnalysis_C, gas_MainCtrl_C)] InOut_list lseq_gassensor_enum) @
-  (enumchansp2_1 [(resume_GasAnalysis_C, resume_MainCtrl_C)] InOut_list) @
-  (enumchansp2_2 [(turn_GasAnalysis_C, turn_MainCtrl_C)] InOut_list Chemical_Angle_list) @
-  (enumchansp2_1 [(stop_GasAnalysis_C, stop_MainCtrl_C)] InOut_list)
+definition rename_MainCtrl_Movement_events where
+"rename_MainCtrl_Movement_events = 
+  (enumchanp2_1 (terminate_Movement_C,terminate_MainCtrl_C) [()]) @
+  (enumchansp2_2 [(gas_Movement_C, gas_MainCtrl_C)] InOut_list lseq_gassensor_enum) @
+  (enumchansp2_1 [(resume_Movement_C, resume_MainCtrl_C)] InOut_list) @
+  (enumchansp2_2 [(turn_Movement_C, turn_MainCtrl_C)] InOut_list Chemical_Angle_list) @
+  (enumchansp2_1 [(stop_Movement_C, stop_MainCtrl_C)] InOut_list)
 "
 
-definition rename_D__GasAnalysis where
-  "rename_D__GasAnalysis idd = rename (set rename_MainCtrl_GasAnalysis_events) (D__GasAnalysis idd)"
+definition rename_D__Movement where
+  "rename_D__Movement idd = rename (set rename_MainCtrl_Movement_events) (D__Movement idd)"
 
 definition D__MainCtrl where
 "D__MainCtrl (idd::integer) = 
   (par_hide
-    (rename_D__GasAnalysis idd)
+    (rename_D__Movement idd)
     {}
     (discard_state (Memory_MainCtrl idd))
   )  \<lbrakk> set [terminate_MainCtrl_C ()] \<Zrres> skip
 "
 
 export_code
-  GasAnalysis_Memory_opt_gs
-  GasAnalysis_MemoryTransitions_opt_0
-  GasAnalysis_MemoryTransitions_opt_1
-  GasAnalysis_MemoryTransitions_opt_2
-  I_GasAnalysis_i1
-  State_GasAnalysis_NoGas
-  State_GasAnalysis_NoGas_R
-  State_GasAnalysis_Analysis_R
-  State_GasAnalysis_GasDetected_R
-  State_GasAnalysis_j1_R
-  State_GasAnalysis_Reading_R
-  MemorySTM_opt_GasAnalysis
-  AUX_opt_GasAnalysis
-  D__GasAnalysis
+  Movement_Memory_opt_gs
+  Movement_MemoryTransitions_opt_0
+  Movement_MemoryTransitions_opt_1
+  Movement_MemoryTransitions_opt_2
+  I_Movement_i1
+  State_Movement_Waiting
+  State_Movement_Waiting_R
+  State_Movement_Analysis_R
+  State_Movement_GasDetected_R
+  State_Movement_j1_R
+  State_Movement_Reading_R
+  MemorySTM_opt_Movement
+  AUX_opt_Movement
+  D__Movement
 in Haskell 
-  (* module_name GasAnalysis *)
+  (* module_name Movement *)
   file_prefix RoboChart_ChemicalDetector 
   (string_classes) 
 
@@ -1851,12 +913,12 @@ subsection \<open> Module \<close>
 chantype Chan_mod0 =
 (* terminates of MainCtrl are mapped to it *)
   terminate_mod0 :: unit 
-(* variable channels: set_x and get_x of GasAnalysis and stm1 are mapped to these channels *)
+(* variable channels: set_x and get_x of Movement and stm1 are mapped to these channels *)
   set_x_mod0 :: core_int
   get_x_mod0 :: core_int
 (* shared variable channels *)
   set_EXT_x_mod0_MainCtrl :: core_int
-(* e1 of GasAnalysis is mapped to it *)
+(* e1 of Movement is mapped to it *)
   e1_mod0 :: "InOut \<times> core_int"
 (* e2 of stm1 is mapped to it *)
   e2_mod0 :: "InOut"
@@ -1932,17 +994,17 @@ definition D__mod0 where
 
 subsection \<open> Export code \<close>
 export_code
-  GasAnalysis_Memory_opt_x
-  GasAnalysis_Memory_opt_l
-  GasAnalysis_MemoryTransitions_opt_0
-  GasAnalysis_MemoryTransitions_opt_1
-  I_GasAnalysis_i0
-  State_GasAnalysis_s0
-  State_GasAnalysis_s0_R
-  STM_GasAnalysis
-  MemorySTM_opt_GasAnalysis 
-  rename_MemorySTM_opt_GasAnalysis
-  D__GasAnalysis 
+  Movement_Memory_opt_x
+  Movement_Memory_opt_l
+  Movement_MemoryTransitions_opt_0
+  Movement_MemoryTransitions_opt_1
+  I_Movement_i0
+  State_Movement_s0
+  State_Movement_s0_R
+  STM_Movement
+  MemorySTM_opt_Movement 
+  rename_MemorySTM_opt_Movement
+  D__Movement 
   stm1_Memory_opt_x
   stm1_MemoryTransitions_opt_0
   I_stm1_i0
@@ -1951,7 +1013,7 @@ export_code
   STM_stm1
   MemorySTM_opt_stm1
   D__stm1
-  rename_D__GasAnalysis
+  rename_D__Movement
   rename_D__stm1
   D__MainCtrl
   rename_D__MainCtrl
