examples/RoboChart/RoboChart_ChemicalDetector_autonomous/RoboChart_ChemicalDetector_autonomous_general.thy
@@ -1,0 +1,182 @@
+
+theory RoboChart_ChemicalDetector_autonomous_general
+  imports "../../../ITree_RoboChart" "../../../RC_Channel_Type" 
+          "../../../Bounded_List"
+begin
+
+subsection \<open> General definitions \<close>
+interpretation rc: robochart_confs "-2" "2" "2" "-2" "2".
+
+subsubsection \<open> Constants \<close>
+
+subsubsection \<open> Types \<close>
+
+(* PrimitiveType in RoboChart like given types in Z, and instantiated in CSP *)
+
+datatype ('a::finite) Chemical_Chem = Chemical_ChemC 'a
+
+abbreviation "Chemical_Chem2_list \<equiv> [Chemical_ChemC (0::2), Chemical_ChemC (1::2)]"
+abbreviation "Chemical_Chem2_set \<equiv> set Chemical_Chem2_list"
+
+definition Chemical_Chem_is_zero::"(2 Chemical_Chem) \<Rightarrow> bool" where
+"Chemical_Chem_is_zero x = (if x = (Chemical_ChemC (0::2)) then True else False)"
+
+value "Chemical_Chem_is_zero (Chemical_ChemC (3::2))"
+
+datatype ('a::finite) Chemical_Intensity = Chemical_IntensityC 'a
+
+abbreviation "Chemical_Intensity2_list \<equiv> [Chemical_IntensityC (0::2), Chemical_IntensityC 1]"
+abbreviation "Chemical_Intensity2_set \<equiv> set Chemical_Intensity2_list"
+
+definition Chemical_Intensity_is_zero::"(2 Chemical_Intensity) \<Rightarrow> bool" where
+"Chemical_Intensity_is_zero x = (if x = (Chemical_IntensityC (0::2)) then True else False)"
+
+fun Chemical_goreq :: "2 Chemical_Intensity \<Rightarrow> 2 Chemical_Intensity \<Rightarrow> bool" where
+"Chemical_goreq (Chemical_IntensityC x) (Chemical_IntensityC y) = (x \<ge> y) "
+
+text \<open> In CSP, LSeq(T,n) from core_defs.csp can be used as a type or an expression. In this 
+RoboChart model, it is used as a type, parametrised by n. We use bounded_list to implement it, 
+such as @{typ "int[2]blist"} for LSeq(int, 2).
+\<close>
+
+fun lseq where
+"lseq s 0 = [[]]" |
+"lseq s (Suc 0) = [[q]. q \<leftarrow> s]" |
+"lseq s (Suc n) = [q # qs. q \<leftarrow> s, qs \<leftarrow> (lseq s n)]"
+
+fun lseqn where
+"lseqn s 0 = lseq s 0" |
+"lseqn s (Suc n) = lseqn s n @ (lseq s (Suc n))"
+
+text \<open> Make a bounded list from the supplied list, a set of all possible elements. \<close>
+definition mk_blist :: "'n itself \<Rightarrow> 'a list \<Rightarrow> ('a['n::finite]blist) list" where
+"mk_blist _ xs = map (bmake TYPE('n)) (lseqn xs CARD('n))"
+
+subsection \<open> Chemical package \<close>
+enumtype Chemical_Status = 
+  Chemical_Status_noGas | Chemical_Status_gasD
+
+abbreviation "Chemical_Status_list \<equiv> enum_Chemical_Status_inst.enum_Chemical_Status"
+abbreviation "Chemical_Status_set \<equiv> set Chemical_Status_list"
+
+enumtype Chemical_Angle = 
+  Chemical_Angle_Left | Chemical_Angle_Right | 
+  Chemical_Angle_Back | Chemical_Angle_Front
+
+abbreviation "Chemical_Angle_list \<equiv> enum_Chemical_Angle_inst.enum_Chemical_Angle"
+abbreviation "Chemical_Angle_set \<equiv> set Chemical_Angle_list"
+
+text \<open> The angle function \<close>
+definition Chemical_angle :: "nat \<Rightarrow> Chemical_Angle" where
+"Chemical_angle x = (if x > 0 then Chemical_Angle_Right else Chemical_Angle_Front)"
+
+record 'a Chemical_GasSensor = 
+  c :: "'a Chemical_Chem"
+  i :: "'a Chemical_Intensity"
+
+type_synonym Chemical_GasSensor2 = "2 Chemical_GasSensor"
+
+definition Chemical_GasSensor2_list :: "Chemical_GasSensor2 list" where 
+"Chemical_GasSensor2_list \<equiv> 
+  [\<lparr>c = cc, i = ii\<rparr>. cc \<leftarrow> Chemical_Chem2_list, ii \<leftarrow> Chemical_Intensity2_list]"
+
+abbreviation "lseq_gassensor_enum \<equiv> mk_blist TYPE(2) Chemical_GasSensor2_list"
+
+(*
+function Chemical_analysis :: "2 Chemical_GasSensor[2]blist \<Rightarrow> Chemical_Status" where
+"Chemical_analysis (bmake TYPE(2) []) =  Chemical_Status_noGas" |
+"Chemical_analysis (bmake TYPE(2) (p#ps)) = 
+  (if Chemical_Chem_is_zero (c p) \<and> (Chemical_analysis (bmake TYPE(2) ps) = Chemical_Status_noGas) 
+   then Chemical_Status_noGas else Chemical_Status_gasD)"
+     apply (auto)
+*)
+
+function Chemical_analysis :: "2 Chemical_GasSensor[2]blist \<Rightarrow> Chemical_Status" where
+"Chemical_analysis (gs) = 
+  (case list_of_blist gs of
+    []      \<Rightarrow> Chemical_Status_noGas |
+    (p#ps)  \<Rightarrow> (if Chemical_Chem_is_zero (c p) \<and> 
+                  (Chemical_analysis (bmake TYPE(2) ps) = Chemical_Status_noGas) 
+                then Chemical_Status_noGas
+                else Chemical_Status_gasD)
+  )"
+  by auto
+
+termination Chemical_analysis 
+  apply (relation "measure (\<lambda> gs. blength gs)")
+  apply (auto)
+proof -
+  fix gs::"2 Chemical_GasSensor [2]blist" and 
+      x21::"2 Chemical_GasSensor" and 
+      x22::"2 Chemical_GasSensor list"
+  assume a1: "list_of_blist gs = x21 # x22"
+  from a1 have f1: "blength gs > 0"
+    by (simp add: blength_def)
+  show "blength (bmake TYPE(2) x22) < blength gs"
+    by (metis a1 blist_remove_head f1 list.sel(3))
+qed
+
+value "Chemical_analysis (bmake TYPE(2) [])"
+value "Chemical_analysis (bmake TYPE(2) [\<lparr>c = Chemical_ChemC (0::2), i = Chemical_IntensityC (0::2)\<rparr>])"
+
+text \<open> The intensity function \<close>
+definition pre_Chemical_intensity :: "2 Chemical_GasSensor[2]blist \<Rightarrow> bool" where
+"pre_Chemical_intensity gs = (blength gs > 0)"
+
+function Chemical_intensity :: "2 Chemical_GasSensor[2]blist \<Rightarrow> (2 Chemical_Intensity)" where
+"Chemical_intensity (gs) = 
+  (case list_of_blist gs of
+    []      \<Rightarrow> Chemical_IntensityC (0::2) |
+    (p#ps)  \<Rightarrow> (if Chemical_goreq (i p) (Chemical_intensity (bmake TYPE(2) ps)) 
+                then i p
+                else Chemical_intensity (bmake TYPE(2) ps))
+  )"
+  by auto
+
+termination Chemical_intensity 
+  apply (relation "measure (\<lambda> gs. blength gs)")
+  apply (auto)
+  by (metis add_Suc_right blength.rep_eq blist_remove_head less_nat_zero_code linorder_cases 
+      list.sel(3) list.size(4) nat.simps(3))+
+
+value "Chemical_intensity (bmake TYPE(2) [])"
+value "Chemical_intensity (bmake TYPE(2) 
+  [\<lparr>c = Chemical_ChemC (0::2), i = Chemical_IntensityC (1::2)\<rparr>,
+   \<lparr>c = Chemical_ChemC (1::2), i = Chemical_IntensityC (0::2)\<rparr>])"
+
+text \<open> The location function \<close>
+definition pre_Chemical_location :: "2 Chemical_GasSensor[2]blist \<Rightarrow> bool" where
+"pre_Chemical_location gs = (blength gs > 0)"
+
+function Chemical_location' :: "2 Chemical_GasSensor[2]blist \<Rightarrow> nat \<Rightarrow> (Chemical_Angle)" where
+"Chemical_location' (gs) x = 
+  (case list_of_blist gs of
+    []      \<Rightarrow> Chemical_angle(x) |
+    (p#ps)  \<Rightarrow> (if (i p) = (Chemical_intensity (gs))
+                then Chemical_angle(x)
+                else Chemical_location' (bmake TYPE(2) ps) (x+1)
+               )
+  )"
+  by auto
+
+termination Chemical_location'
+  apply (relation "measure (\<lambda> (gs, n). blength gs)")
+  apply (auto)
+  by (metis add_Suc_right blength.rep_eq blist_remove_head less_nat_zero_code linorder_cases 
+      list.sel(3) list.size(4) nat.simps(3))+
+
+abbreviation "Chemical_location gs \<equiv> Chemical_location' gs 0"
+
+value "Chemical_location (bmake TYPE(2) [])"
+value "Chemical_location (bmake TYPE(2) 
+  [\<lparr>c = Chemical_ChemC (0::2), i = Chemical_IntensityC (0::2)\<rparr>,
+   \<lparr>c = Chemical_ChemC (1::2), i = Chemical_IntensityC (1::2)\<rparr>])"
+
+subsection \<open> Location package \<close>
+enumtype Location_Loc = 
+  Location_Loc_left | Location_Loc_right | Location_Loc_front
+
+definition "Location_Loc_list = enum_Location_Loc_inst.enum_Location_Loc"
+definition "Location_Loc_set = set Location_Loc_list"
+
+end
