examples/RoboChart/RoboChart_ChemicalDetector_autonomous/RoboChart_ChemicalDetector_autonomous_maincontroller.thy
@@ -1,0 +1,863 @@
+
+theory RoboChart_ChemicalDetector_autonomous_maincontroller
+  imports "RoboChart_ChemicalDetector_autonomous_general"
+begin
+
+subsection \<open> GasAnalysis \<close>
+definition "const_GasAnalysis_thr \<equiv> Chemical_IntensityC (1::2)"
+
+enumtype SIDS_GasAnalysis = SID_GasAnalysis
+	              | SID_GasAnalysis_NoGas
+	              | SID_GasAnalysis_Analysis
+	              | SID_GasAnalysis_GasDetected
+	              | SID_GasAnalysis_j1
+	              | SID_GasAnalysis_Reading
+
+definition "SIDS_GasAnalysis_list = enum_SIDS_GasAnalysis_inst.enum_SIDS_GasAnalysis"
+definition "SIDS_GasAnalysis_set = set SIDS_GasAnalysis_list"
+definition "SIDS_GasAnalysis_nodes = (removeAll SID_GasAnalysis SIDS_GasAnalysis_list)"
+definition "SIDS_GasAnalysis_no_NoGas = (removeAll SID_GasAnalysis_NoGas SIDS_GasAnalysis_list)"
+definition "SIDS_GasAnalysis_no_Analysis = (removeAll SID_GasAnalysis_Analysis SIDS_GasAnalysis_list)"
+definition "SIDS_GasAnalysis_no_GasDetected = (removeAll SID_GasAnalysis_GasDetected SIDS_GasAnalysis_list)"
+definition "SIDS_GasAnalysis_no_Reading = (removeAll SID_GasAnalysis_Reading SIDS_GasAnalysis_list)"
+definition "SIDS_GasAnalysis_no_j1 = (removeAll SID_GasAnalysis_j1 SIDS_GasAnalysis_list)"
+
+enumtype TIDS_GasAnalysis = NULLTRANSITION__GasAnalysis
+	              | TID_GasAnalysis_t1
+	              | TID_GasAnalysis_t2
+	              | TID_GasAnalysis_t3
+	              | TID_GasAnalysis_t4
+	              | TID_GasAnalysis_t8
+	              | TID_GasAnalysis_t9a
+	              | TID_GasAnalysis_t0
+
+definition "TIDS_GasAnalysis_list = enum_TIDS_GasAnalysis_inst.enum_TIDS_GasAnalysis"
+definition "TIDS_GasAnalysis_set = set TIDS_GasAnalysis_list"
+
+text \<open> Identifiers of transitions that can interrupt a state, excluding transitions from junctions. \<close>
+definition "ITIDS_GasAnalysis_list = [TID_GasAnalysis_t0, 
+  TID_GasAnalysis_t2, TID_GasAnalysis_t3,	TID_GasAnalysis_t4,	
+  TID_GasAnalysis_t8,	TID_GasAnalysis_t9a
+]"
+
+definition "ITIDS_GasAnalysis = set ITIDS_GasAnalysis_list"
+
+chantype Chan_GasAnalysis =
+(* flow channels *)
+  internal_GasAnalysis :: TIDS_GasAnalysis
+  enter_GasAnalysis :: "SIDS_GasAnalysis \<times> SIDS_GasAnalysis"
+  entered_GasAnalysis :: "SIDS_GasAnalysis \<times> SIDS_GasAnalysis"
+  exit_GasAnalysis :: "SIDS_GasAnalysis \<times> SIDS_GasAnalysis"
+  exited_GasAnalysis :: "SIDS_GasAnalysis \<times> SIDS_GasAnalysis"
+  terminate_GasAnalysis :: unit
+
+(* Variables *)
+  get_st_GasAnalysis :: Chemical_Status
+  set_st_GasAnalysis :: Chemical_Status
+  get_gs_GasAnalysis :: "2 Chemical_GasSensor[2]blist" (* "Chemical_GasSensor LSeq"*)
+  set_gs_GasAnalysis :: "2 Chemical_GasSensor[2]blist"
+  get_i_GasAnalysis :: "2 Chemical_Intensity"
+  set_i_GasAnalysis :: "2 Chemical_Intensity"
+  get_a_GasAnalysis :: "Chemical_Angle"
+  set_a_GasAnalysis :: "Chemical_Angle"
+
+(* event channels *)
+  gas__GasAnalysis :: "TIDS_GasAnalysis \<times> InOut \<times> 2 Chemical_GasSensor[2]blist"
+  gas_GasAnalysis :: "InOut \<times> 2 Chemical_GasSensor[2]blist"
+  resume__GasAnalysis :: "TIDS_GasAnalysis \<times> InOut"
+  resume_GasAnalysis :: "InOut"
+  turn__GasAnalysis :: "TIDS_GasAnalysis \<times> InOut \<times> Chemical_Angle"
+  turn_GasAnalysis :: "InOut \<times> Chemical_Angle"
+  stop__GasAnalysis :: "TIDS_GasAnalysis \<times> InOut"
+  stop_GasAnalysis :: "InOut"
+
+subsubsection \<open> Sets of events \<close>
+(* How to use a list to represent all possible values of Chemical_GasSensor[2]blist *)
+term "\<lbrace>gas__GasAnalysis (t, d, s). t \<in> set [TID_GasAnalysis_t0, TID_GasAnalysis_t2, 
+     TID_GasAnalysis_t3, TID_GasAnalysis_t4,
+     TID_GasAnalysis_t8, TID_GasAnalysis_t9a] \<and> d \<in> set [din, dout] \<and> s \<in> set lseq_gassensor_enum\<rbrace> \<union> {}"
+definition int_int_GasAnalysis' where
+"int_int_GasAnalysis' = set (
+  (enumchans3 [gas__GasAnalysis_C] 
+    [TID_GasAnalysis_t0, TID_GasAnalysis_t2, 
+     TID_GasAnalysis_t3, TID_GasAnalysis_t4,
+     TID_GasAnalysis_t8, TID_GasAnalysis_t9a] 
+    [din, dout] 
+    (lseq_gassensor_enum)) @
+  (enumchans2 [resume__GasAnalysis_C] 
+    [TID_GasAnalysis_t0, TID_GasAnalysis_t2, 
+     TID_GasAnalysis_t3, TID_GasAnalysis_t4,
+     TID_GasAnalysis_t8, TID_GasAnalysis_t9a] 
+    [din, dout]) @
+  (enumchans3 [turn__GasAnalysis_C] 
+    [TID_GasAnalysis_t0, TID_GasAnalysis_t2, 
+     TID_GasAnalysis_t3, TID_GasAnalysis_t4,
+     TID_GasAnalysis_t8, TID_GasAnalysis_t9a] 
+    [din, dout]
+    Chemical_Angle_list
+    ) @
+  (enumchans2 [stop__GasAnalysis_C] 
+    [TID_GasAnalysis_t0, TID_GasAnalysis_t2, 
+     TID_GasAnalysis_t3, TID_GasAnalysis_t4,
+     TID_GasAnalysis_t8, TID_GasAnalysis_t9a] 
+    [din, dout]  
+    ) @
+  (enumchan1 internal_GasAnalysis_C 
+    [TID_GasAnalysis_t0, TID_GasAnalysis_t2, 
+     TID_GasAnalysis_t3, TID_GasAnalysis_t4,
+     TID_GasAnalysis_t8, TID_GasAnalysis_t9a])
+)"
+
+definition int_int_GasAnalysis where
+"int_int_GasAnalysis = set (
+  (enumchans3 [gas__GasAnalysis_C] 
+    [TID_GasAnalysis_t0, TID_GasAnalysis_t2, 
+     TID_GasAnalysis_t3, TID_GasAnalysis_t4,
+     TID_GasAnalysis_t8, TID_GasAnalysis_t9a] 
+    [din, dout] 
+    (lseq_gassensor_enum)) @
+  (enumchans2 [resume__GasAnalysis_C] 
+    [TID_GasAnalysis_t0, TID_GasAnalysis_t2, 
+     TID_GasAnalysis_t3, TID_GasAnalysis_t4,
+     TID_GasAnalysis_t8, TID_GasAnalysis_t9a] 
+    [din, dout]) @
+  (enumchans3 [turn__GasAnalysis_C] 
+    [TID_GasAnalysis_t0, TID_GasAnalysis_t2, 
+     TID_GasAnalysis_t3, TID_GasAnalysis_t4,
+     TID_GasAnalysis_t8, TID_GasAnalysis_t9a] 
+    [din, dout]
+    Chemical_Angle_list
+    ) @
+  (enumchans2 [stop__GasAnalysis_C] 
+    [TID_GasAnalysis_t0, TID_GasAnalysis_t2, 
+     TID_GasAnalysis_t3, TID_GasAnalysis_t4,
+     TID_GasAnalysis_t8, TID_GasAnalysis_t9a] 
+    [din, dout]  
+    ) @
+  (enumchan1 internal_GasAnalysis_C 
+    [TID_GasAnalysis_t0, TID_GasAnalysis_t2, 
+     TID_GasAnalysis_t3, TID_GasAnalysis_t4,
+     TID_GasAnalysis_t8, TID_GasAnalysis_t9a])
+)"
+
+abbreviation "enter_exit_channels_GasAnalysis \<equiv>
+  [enter_GasAnalysis_C, entered_GasAnalysis_C, exit_GasAnalysis_C, exited_GasAnalysis_C]"
+
+definition internal_events_GasAnalysis where
+"internal_events_GasAnalysis = set (
+  enumchans2 enter_exit_channels_GasAnalysis SIDS_GasAnalysis_list SIDS_GasAnalysis_list
+)"
+
+
+definition GasAnalysis_i_events where
+"GasAnalysis_i_events = 
+    set (enumchans1 [get_i_GasAnalysis_C, set_i_GasAnalysis_C] Chemical_Intensity2_list)
+"
+
+definition GasAnalysis_st_events where
+"GasAnalysis_st_events = 
+    set (enumchans1 [get_st_GasAnalysis_C, set_st_GasAnalysis_C] Chemical_Status_list)
+"
+
+definition GasAnalysis_gs_events where
+"GasAnalysis_gs_events = 
+    set (enumchans1 [get_gs_GasAnalysis_C, set_gs_GasAnalysis_C] lseq_gassensor_enum)
+"
+
+definition GasAnalysis_a_events where
+"GasAnalysis_a_events = 
+    set (enumchans1 [get_a_GasAnalysis_C, set_a_GasAnalysis_C] Chemical_Angle_list)
+"
+
+definition GasAnalysis_MachineInternalEvents where
+"GasAnalysis_MachineInternalEvents = 
+  set (enumchan1 internal_GasAnalysis_C TIDS_GasAnalysis_list)
+"
+
+subsubsection \<open> State Machine Memory \<close>
+text \<open> Memory cell processes \<close>
+
+(* for the local variable x *)
+definition GasAnalysis_Memory_opt_gs where
+"GasAnalysis_Memory_opt_gs = 
+  mem_of_lvar get_gs_GasAnalysis set_gs_GasAnalysis 
+    (set (lseq_gassensor_enum))"
+
+definition GasAnalysis_Memory_opt_a where
+"GasAnalysis_Memory_opt_a = mem_of_lvar get_a_GasAnalysis set_a_GasAnalysis Chemical_Angle_set"
+
+definition GasAnalysis_Memory_opt_i where
+"GasAnalysis_Memory_opt_i = mem_of_lvar get_i_GasAnalysis set_i_GasAnalysis (Chemical_Intensity2_set)"
+
+definition GasAnalysis_Memory_opt_st where
+"GasAnalysis_Memory_opt_st = mem_of_lvar get_st_GasAnalysis set_st_GasAnalysis (Chemical_Status_set)"
+
+text \<open> Memory transition processes \<close>
+definition GasAnalysis_MemoryTransitions_opt_0 where
+"GasAnalysis_MemoryTransitions_opt_0 = 
+  loop (\<lambda> id::integer. 
+    (do {outp internal_GasAnalysis TID_GasAnalysis_t1 ; Ret (id)} \<box> 
+     do {gs \<leftarrow> inp_in gas__GasAnalysis (set [(TID_GasAnalysis_t2, din, x). 
+              x \<leftarrow> (lseq_gassensor_enum)]) ; Ret (id)}  \<box> 
+     do {gs \<leftarrow> inp_in gas__GasAnalysis (set [(TID_GasAnalysis_t0, din, x). 
+              x \<leftarrow> (lseq_gassensor_enum)]) ; Ret (id)})
+  )
+"
+
+definition GasAnalysis_MemoryTransitions_opt_1 where
+"GasAnalysis_MemoryTransitions_opt_1 = 
+  loop (\<lambda> id::integer.
+    do {st \<leftarrow> inp_in get_st_GasAnalysis Chemical_Status_set ; 
+      (
+        do {guard (st = Chemical_Status_gasD); outp internal_GasAnalysis TID_GasAnalysis_t4 ; Ret (id)} \<box>
+        do {guard (st = Chemical_Status_noGas); outp internal_GasAnalysis TID_GasAnalysis_t3 ; Ret (id)} \<box>
+        do {x \<leftarrow> inp_in set_st_GasAnalysis Chemical_Status_set; Ret (id)}
+      )
+    }
+  )
+"
+
+definition GasAnalysis_MemoryTransitions_opt_2 where
+"GasAnalysis_MemoryTransitions_opt_2 = 
+  loop (\<lambda> id::integer.
+    do {i \<leftarrow> inp_in get_i_GasAnalysis Chemical_Intensity2_set ; 
+      (
+        do {guard (\<not> (Chemical_goreq i const_GasAnalysis_thr)); outp internal_GasAnalysis TID_GasAnalysis_t9a ; Ret (id)} \<box>
+        do {guard (Chemical_goreq i const_GasAnalysis_thr); outp internal_GasAnalysis TID_GasAnalysis_t8 ; Ret (id)} \<box>
+        do {x \<leftarrow> inp_in set_i_GasAnalysis Chemical_Intensity2_set; Ret (id)}
+      )
+    }
+  )
+"
+
+subsubsection \<open> States \<close>
+paragraph \<open> Initial \<close>
+definition I_GasAnalysis_i1 where
+"I_GasAnalysis_i1 = (\<lambda> (id::integer) . 
+  do {outp internal_GasAnalysis TID_GasAnalysis_t1 ; 
+      outp enter_GasAnalysis (SID_GasAnalysis, SID_GasAnalysis_NoGas);
+      outp entered_GasAnalysis (SID_GasAnalysis, SID_GasAnalysis_NoGas)
+  })
+"
+
+paragraph \<open> NoGas \<close>
+definition CS_GasAnalysis_NoGas_sync where
+"CS_GasAnalysis_NoGas_sync = 
+  set (
+      \<comment> \<open> enter from x to y \<close>
+      (enumchans2 enter_exit_channels_GasAnalysis [SID_GasAnalysis_NoGas] SIDS_GasAnalysis_nodes)@
+      \<comment> \<open> enter from y to x \<close>
+      (enumchans2 enter_exit_channels_GasAnalysis SIDS_GasAnalysis_nodes [SID_GasAnalysis_NoGas])
+)"
+
+definition GasAnalysis_NoGas_triggers where
+"GasAnalysis_NoGas_triggers = set (
+  (enumchan1 internal_GasAnalysis_C 
+    [TID_GasAnalysis_t3, TID_GasAnalysis_t4,
+     TID_GasAnalysis_t8, TID_GasAnalysis_t9a]) @
+  (enumchans3 [gas__GasAnalysis_C] 
+    [TID_GasAnalysis_t0, TID_GasAnalysis_t2] 
+    [din, dout] 
+    (lseq_gassensor_enum))
+)
+"
+
+definition tids_GasAnalysis_NoGas where
+" tids_GasAnalysis_NoGas = 
+    (filter 
+        (\<lambda> s. s \<notin> {NULLTRANSITION__GasAnalysis, TID_GasAnalysis_t9a,
+          TID_GasAnalysis_t8, TID_GasAnalysis_t4, TID_GasAnalysis_t3, 
+          TID_GasAnalysis_t2, TID_GasAnalysis_t0}) 
+        ITIDS_GasAnalysis_list)"
+
+abbreviation Other_SIDs_to_NoGas_GasAnalysis where
+"Other_SIDs_to_NoGas_GasAnalysis \<equiv>
+  set [(s, SID_GasAnalysis_NoGas) . s \<leftarrow> (SIDS_GasAnalysis_no_NoGas)]"
+
+definition 
+"exit_events_GasAnalysis idd sid tids other_sids =
+    (do {inp_in internal_GasAnalysis (set tids);
+        y \<leftarrow> inp_in exit_GasAnalysis other_sids;
+          outp exited_GasAnalysis (fst y, sid);
+          Ret(False, idd, sid)
+        } \<box>
+    do {t \<leftarrow> inp_in gas__GasAnalysis (set [(t, d, gs). 
+            t \<leftarrow> (tids), d \<leftarrow> InOut_list,
+            gs \<leftarrow> (lseq_gassensor_enum)]) ;
+          y \<leftarrow> inp_in exit_GasAnalysis other_sids;
+            outp exited_GasAnalysis (fst y, sid);
+            Ret(False, idd, sid)
+        } \<box>
+    do {t \<leftarrow> inp_in resume__GasAnalysis (set [(t, d). 
+            t \<leftarrow> (tids), d \<leftarrow> InOut_list]) ;
+          y \<leftarrow> inp_in exit_GasAnalysis other_sids;
+            outp exited_GasAnalysis (fst y, sid);
+            Ret(False, idd, sid)
+        } \<box>
+    do {t \<leftarrow> inp_in turn__GasAnalysis (set [(t, d, a). 
+            t \<leftarrow> (tids), d \<leftarrow> InOut_list,
+            a \<leftarrow> Chemical_Angle_list]) ;
+          y \<leftarrow> inp_in exit_GasAnalysis other_sids;
+            outp exited_GasAnalysis (fst y, sid);
+            Ret(False, idd, sid)
+        } \<box>
+    do {t \<leftarrow> inp_in stop__GasAnalysis (set [(t, d). 
+            t \<leftarrow> (tids), d \<leftarrow> InOut_list]) ;
+          y \<leftarrow> inp_in exit_GasAnalysis other_sids;
+            outp exited_GasAnalysis (fst y, sid);
+            Ret(False, idd, sid)
+        }
+    )"
+
+definition State_GasAnalysis_NoGas where 
+"State_GasAnalysis_NoGas = 
+  loop (\<lambda> (id::integer).
+    do {sd \<leftarrow> inp_in enter_GasAnalysis Other_SIDs_to_NoGas_GasAnalysis ; 
+        \<comment> \<open> State passed to next loop, including a condition initially True. \<close>
+        ret \<leftarrow> Ret (True, id, fst sd) ; 
+        \<comment> \<open> State_GasAnalysis_NoGas_execute \<close>
+        (iterate 
+           \<comment> \<open> condition \<close>
+           (\<lambda> s. fst s) 
+           \<comment> \<open> P \<close>
+           (\<lambda> s.
+            do {
+              outp entered_GasAnalysis (snd (snd s), SID_GasAnalysis_NoGas);
+              (do {skip ; stop} \<triangle>
+                (
+                \<comment> \<open> T_GasAnalysis_t2 \<close>
+                do {t \<leftarrow> inp_in gas__GasAnalysis (set [(TID_GasAnalysis_t2, din, gs). 
+                                gs \<leftarrow> (lseq_gassensor_enum)]) ;
+                      outp set_gs_GasAnalysis (snd (snd t)) ; 
+                      outp exit_GasAnalysis (SID_GasAnalysis_NoGas, SID_GasAnalysis_NoGas);
+                      outp exited_GasAnalysis (SID_GasAnalysis_NoGas, SID_GasAnalysis_NoGas);
+                      outp enter_GasAnalysis (SID_GasAnalysis_NoGas, SID_GasAnalysis_Analysis);
+                      outp entered_GasAnalysis (SID_GasAnalysis_NoGas, SID_GasAnalysis_Analysis);
+                      Ret(False, fst (snd s), SID_GasAnalysis_NoGas)
+                    } \<box>
+                (exit_events_GasAnalysis (fst (snd s)) SID_GasAnalysis_NoGas 
+                   tids_GasAnalysis_NoGas Other_SIDs_to_NoGas_GasAnalysis)
+                )
+              )
+            })
+            \<comment> \<open> The previous state: a triple \<close> 
+            (ret)
+        ) ;
+        Ret (id)
+  }
+)
+"
+
+definition State_GasAnalysis_NoGas_R where
+"State_GasAnalysis_NoGas_R (idd::integer) = 
+   (discard_state (State_GasAnalysis_NoGas idd)) \<comment> \<open> discard state to match with skip on the right\<close>
+    \<parallel>\<^bsub> (int_int_GasAnalysis - GasAnalysis_NoGas_triggers) \<^esub> 
+   skip
+"
+
+paragraph \<open> Analysis \<close>
+definition CS_GasAnalysis_Analysis_sync where
+"CS_GasAnalysis_Analysis_sync = 
+  set (
+      \<comment> \<open> enter from x to y \<close>
+      (enumchans2 enter_exit_channels_GasAnalysis [SID_GasAnalysis_Analysis] SIDS_GasAnalysis_nodes)@
+      \<comment> \<open> enter from y to x \<close>
+      (enumchans2 enter_exit_channels_GasAnalysis SIDS_GasAnalysis_nodes [SID_GasAnalysis_Analysis])
+)"
+
+definition GasAnalysis_Analysis_triggers where
+"GasAnalysis_Analysis_triggers = set (
+  (enumchan1 internal_GasAnalysis_C 
+    [TID_GasAnalysis_t3, TID_GasAnalysis_t4,
+     TID_GasAnalysis_t8, TID_GasAnalysis_t9a]) @
+  (enumchans3 [gas__GasAnalysis_C] 
+    [TID_GasAnalysis_t0, TID_GasAnalysis_t2] 
+    [din, dout] 
+    (lseq_gassensor_enum))
+)
+"
+
+definition tids_GasAnalysis_Analysis where
+" tids_GasAnalysis_Analysis = 
+    (filter 
+        (\<lambda> s. s \<notin> {NULLTRANSITION__GasAnalysis, TID_GasAnalysis_t9a,
+          TID_GasAnalysis_t8, TID_GasAnalysis_t4, TID_GasAnalysis_t3, 
+          TID_GasAnalysis_t2, TID_GasAnalysis_t0}) 
+        ITIDS_GasAnalysis_list)"
+
+abbreviation Other_SIDs_to_Analysis_GasAnalysis where
+"Other_SIDs_to_Analysis_GasAnalysis \<equiv> 
+  set [(s, SID_GasAnalysis_Analysis) . s \<leftarrow> (SIDS_GasAnalysis_no_Analysis)]"
+
+definition State_GasAnalysis_Analysis where 
+"State_GasAnalysis_Analysis = 
+  loop (\<lambda> (id::integer).
+    do {sd \<leftarrow> inp_in enter_GasAnalysis Other_SIDs_to_Analysis_GasAnalysis ; 
+        \<comment> \<open> State passed to next loop, including a condition initially True. \<close>
+        ret \<leftarrow> Ret (True, id, fst sd) ; 
+        \<comment> \<open> State_GasAnalysis_Analysis_execute \<close>
+        (iterate 
+           \<comment> \<open> condition \<close>
+           (\<lambda> s. fst s) 
+           \<comment> \<open> P \<close>
+           (\<lambda> s.
+            do {
+              gs \<leftarrow> inp_in get_gs_GasAnalysis (set (lseq_gassensor_enum));
+              outp set_st_GasAnalysis (Chemical_analysis gs);
+              outp entered_GasAnalysis (snd (snd s), SID_GasAnalysis_Analysis);
+              (do {skip ; stop} \<triangle>
+                (
+                \<comment> \<open> T_GasAnalysis_t3 \<close>
+                do {outp internal_GasAnalysis TID_GasAnalysis_t3 ;
+                    outp exit_GasAnalysis (SID_GasAnalysis_Analysis, SID_GasAnalysis_Analysis);
+                    outp exited_GasAnalysis (SID_GasAnalysis_Analysis, SID_GasAnalysis_Analysis);
+                    outp resume_GasAnalysis dout;
+                    outp enter_GasAnalysis (SID_GasAnalysis_Analysis, SID_GasAnalysis_NoGas);
+                    outp entered_GasAnalysis (SID_GasAnalysis_Analysis, SID_GasAnalysis_NoGas);
+                    Ret(False, fst (snd s), SID_GasAnalysis_Analysis)
+                    } \<box>
+                \<comment> \<open> T_GasAnalysis_t4 \<close>
+                do {outp internal_GasAnalysis TID_GasAnalysis_t4 ;
+                    outp exit_GasAnalysis (SID_GasAnalysis_Analysis, SID_GasAnalysis_Analysis);
+                    outp exited_GasAnalysis (SID_GasAnalysis_Analysis, SID_GasAnalysis_Analysis);
+                    outp enter_GasAnalysis (SID_GasAnalysis_Analysis, SID_GasAnalysis_GasDetected);
+                    outp entered_GasAnalysis (SID_GasAnalysis_Analysis, SID_GasAnalysis_GasDetected);
+                    Ret(False, fst (snd s), SID_GasAnalysis_Analysis)
+                    } \<box>
+                (exit_events_GasAnalysis (fst (snd s)) SID_GasAnalysis_Analysis 
+                   tids_GasAnalysis_Analysis Other_SIDs_to_Analysis_GasAnalysis)
+                )
+              )
+            })
+            \<comment> \<open> The previous state: a triple \<close> 
+            (ret)
+        ) ;
+        Ret (id)
+  }
+)
+"
+
+definition State_GasAnalysis_Analysis_R where
+"State_GasAnalysis_Analysis_R (idd::integer) = 
+   (discard_state (State_GasAnalysis_Analysis idd)) \<comment> \<open> discard state to match with skip on the right\<close>
+    \<parallel>\<^bsub> (int_int_GasAnalysis - GasAnalysis_Analysis_triggers) \<^esub> 
+   skip
+"
+
+paragraph \<open> GasDetected \<close>
+definition CS_GasAnalysis_GasDetected_sync where
+"CS_GasAnalysis_GasDetected_sync = 
+  set (
+      \<comment> \<open> enter from x to y \<close>
+      (enumchans2 enter_exit_channels_GasAnalysis [SID_GasAnalysis_GasDetected] SIDS_GasAnalysis_nodes)@
+      \<comment> \<open> enter from y to x \<close>
+      (enumchans2 enter_exit_channels_GasAnalysis SIDS_GasAnalysis_nodes [SID_GasAnalysis_GasDetected])
+)"
+
+definition GasAnalysis_GasDetected_triggers where
+"GasAnalysis_GasDetected_triggers = set (
+  (enumchan1 internal_GasAnalysis_C 
+    [TID_GasAnalysis_t3, TID_GasAnalysis_t4,
+     TID_GasAnalysis_t8, TID_GasAnalysis_t9a]) @
+  (enumchans3 [gas__GasAnalysis_C] 
+    [TID_GasAnalysis_t0, TID_GasAnalysis_t2] 
+    [din, dout] 
+    (lseq_gassensor_enum))
+)
+"
+
+definition tids_GasAnalysis_GasDetected where
+" tids_GasAnalysis_GasDetected = 
+    (filter 
+        (\<lambda> s. s \<notin> {NULLTRANSITION__GasAnalysis, TID_GasAnalysis_t9a,
+          TID_GasAnalysis_t8, TID_GasAnalysis_t4, TID_GasAnalysis_t3, 
+          TID_GasAnalysis_t2, TID_GasAnalysis_t0}) 
+        ITIDS_GasAnalysis_list)"
+
+abbreviation Other_SIDs_to_GasDetected_GasAnalysis where
+"Other_SIDs_to_GasDetected_GasAnalysis \<equiv>
+  set [(s, SID_GasAnalysis_GasDetected) . s \<leftarrow> (SIDS_GasAnalysis_no_GasDetected)]"
+
+definition State_GasAnalysis_GasDetected where 
+"State_GasAnalysis_GasDetected = 
+  loop (\<lambda> (id::integer).
+    do {sd \<leftarrow> inp_in enter_GasAnalysis Other_SIDs_to_GasDetected_GasAnalysis ; 
+        \<comment> \<open> State passed to next loop, including a condition initially True. \<close>
+        ret \<leftarrow> Ret (True, id, fst sd) ; 
+        \<comment> \<open> State_GasAnalysis_GasDetected_execute \<close>
+        (iterate 
+           \<comment> \<open> condition \<close>
+           (\<lambda> s. fst s) 
+           \<comment> \<open> P \<close>
+           (\<lambda> s.
+            do {
+              gs \<leftarrow> inp_in get_gs_GasAnalysis (set (lseq_gassensor_enum));
+              guard (pre_Chemical_intensity(gs));
+              outp set_i_GasAnalysis (Chemical_intensity gs);
+              outp entered_GasAnalysis (snd (snd s), SID_GasAnalysis_GasDetected);
+              (do {skip ; stop} \<triangle>
+                (
+                \<comment> \<open> T_GasAnalysis_t8 \<close>
+                do {outp internal_GasAnalysis TID_GasAnalysis_t8 ;
+                    outp exit_GasAnalysis (SID_GasAnalysis_GasDetected, SID_GasAnalysis_GasDetected);
+                    outp exited_GasAnalysis (SID_GasAnalysis_GasDetected, SID_GasAnalysis_GasDetected);
+                    outp stop_GasAnalysis dout;
+                    outp enter_GasAnalysis (SID_GasAnalysis_GasDetected, SID_GasAnalysis_j1);
+                    outp entered_GasAnalysis (SID_GasAnalysis_GasDetected, SID_GasAnalysis_j1);
+                    Ret(False, fst (snd s), SID_GasAnalysis_GasDetected)
+                    } \<box>
+                 \<comment> \<open> T_GasAnalysis_t9a \<close>
+                do {outp internal_GasAnalysis TID_GasAnalysis_t9a ;
+                    outp exit_GasAnalysis (SID_GasAnalysis_GasDetected, SID_GasAnalysis_GasDetected);
+                    outp exited_GasAnalysis (SID_GasAnalysis_GasDetected, SID_GasAnalysis_GasDetected);
+                    gs \<leftarrow> inp_in get_gs_GasAnalysis (set (lseq_gassensor_enum));
+                    guard (pre_Chemical_location(gs));
+                    outp set_a_GasAnalysis (Chemical_location gs);
+                    a \<leftarrow> inp_in get_a_GasAnalysis Chemical_Angle_set;
+                    outp turn_GasAnalysis (dout, a);
+                    outp enter_GasAnalysis (SID_GasAnalysis_GasDetected, SID_GasAnalysis_Reading);
+                    outp entered_GasAnalysis (SID_GasAnalysis_GasDetected, SID_GasAnalysis_Reading);
+                    Ret(False, fst (snd s), SID_GasAnalysis_GasDetected)
+                    } \<box>
+                (exit_events_GasAnalysis (fst (snd s)) SID_GasAnalysis_GasDetected 
+                   tids_GasAnalysis_GasDetected Other_SIDs_to_GasDetected_GasAnalysis)
+                )
+              )
+            })
+            \<comment> \<open> The previous state: a triple \<close> 
+            (ret)
+        ) ;
+        Ret (id)
+  }
+)
+"
+
+definition State_GasAnalysis_GasDetected_R where
+"State_GasAnalysis_GasDetected_R (idd::integer) = 
+   (discard_state (State_GasAnalysis_GasDetected idd)) \<comment> \<open> discard state to match with skip on the right\<close>
+    \<parallel>\<^bsub> (int_int_GasAnalysis - GasAnalysis_GasDetected_triggers) \<^esub> 
+   skip
+"
+
+paragraph \<open> Final \<close>
+definition CS_GasAnalysis_j1_sync where
+"CS_GasAnalysis_j1_sync = 
+  set (
+      \<comment> \<open> enter from x to y \<close>
+      (enumchans2 enter_exit_channels_GasAnalysis [SID_GasAnalysis_j1] SIDS_GasAnalysis_nodes)@
+      \<comment> \<open> enter from y to x \<close>
+      (enumchans2 enter_exit_channels_GasAnalysis SIDS_GasAnalysis_nodes [SID_GasAnalysis_j1])
+)"
+
+definition GasAnalysis_j1_triggers where
+"GasAnalysis_j1_triggers = set ([])
+"
+
+definition tids_GasAnalysis_j1 where
+" tids_GasAnalysis_j1 = 
+    (filter 
+        (\<lambda> s. s \<notin> {NULLTRANSITION__GasAnalysis, TID_GasAnalysis_t9a,
+          TID_GasAnalysis_t8, TID_GasAnalysis_t4, TID_GasAnalysis_t3, 
+          TID_GasAnalysis_t2, TID_GasAnalysis_t0}) 
+        ITIDS_GasAnalysis_list)"
+
+abbreviation Other_SIDs_to_j1_GasAnalysis where
+"Other_SIDs_to_j1_GasAnalysis \<equiv>
+  set [(s, SID_GasAnalysis_j1) . s \<leftarrow> (SIDS_GasAnalysis_no_j1)]"
+
+definition State_GasAnalysis_j1 where 
+"State_GasAnalysis_j1 = 
+  loop (\<lambda> (id::integer).
+    do {sd \<leftarrow> inp_in enter_GasAnalysis Other_SIDs_to_j1_GasAnalysis ; 
+        outp terminate_GasAnalysis ();
+        Ret (id)
+    }
+)
+"
+
+definition State_GasAnalysis_j1_R where
+"State_GasAnalysis_j1_R (idd::integer) = 
+   (discard_state (State_GasAnalysis_j1 idd)) \<comment> \<open> discard state to match with skip on the right\<close>
+    \<parallel>\<^bsub> (int_int_GasAnalysis - GasAnalysis_j1_triggers) \<^esub> 
+   skip
+"
+
+paragraph \<open> Reading \<close>
+definition CS_GasAnalysis_Reading_sync where
+"CS_GasAnalysis_Reading_sync = 
+  set (
+      \<comment> \<open> enter from x to y \<close>
+      (enumchans2 enter_exit_channels_GasAnalysis [SID_GasAnalysis_Reading] SIDS_GasAnalysis_nodes)@
+      \<comment> \<open> enter from y to x \<close>
+      (enumchans2 enter_exit_channels_GasAnalysis SIDS_GasAnalysis_nodes [SID_GasAnalysis_Reading])
+)"
+
+definition GasAnalysis_Reading_triggers where
+"GasAnalysis_Reading_triggers = set (
+  (enumchan1 internal_GasAnalysis_C 
+    [TID_GasAnalysis_t3, TID_GasAnalysis_t4,
+     TID_GasAnalysis_t8, TID_GasAnalysis_t9a]) @
+  (enumchans3 [gas__GasAnalysis_C] 
+    [TID_GasAnalysis_t0, TID_GasAnalysis_t2] 
+    [din, dout] 
+    (lseq_gassensor_enum))
+)
+"
+
+definition tids_GasAnalysis_Reading where
+" tids_GasAnalysis_Reading = 
+    (filter 
+        (\<lambda> s. s \<notin> {NULLTRANSITION__GasAnalysis, TID_GasAnalysis_t9a,
+          TID_GasAnalysis_t8, TID_GasAnalysis_t4, TID_GasAnalysis_t3, 
+          TID_GasAnalysis_t2, TID_GasAnalysis_t0}) 
+        ITIDS_GasAnalysis_list)"
+
+abbreviation Other_SIDs_to_Reading_GasAnalysis where
+"Other_SIDs_to_Reading_GasAnalysis \<equiv>
+  set [(s, SID_GasAnalysis_Reading) . s \<leftarrow> (SIDS_GasAnalysis_no_Reading)]"
+
+definition State_GasAnalysis_Reading where 
+"State_GasAnalysis_Reading = 
+  loop (\<lambda> (id::integer).
+    do {sd \<leftarrow> inp_in enter_GasAnalysis Other_SIDs_to_Reading_GasAnalysis ; 
+        \<comment> \<open> State passed to next loop, including a condition initially True. \<close>
+        ret \<leftarrow> Ret (True, id, fst sd) ; 
+        \<comment> \<open> State_GasAnalysis_Reading_execute \<close>
+        (iterate 
+           \<comment> \<open> condition \<close>
+           (\<lambda> s. fst s) 
+           \<comment> \<open> P \<close>
+           (\<lambda> s.
+            do {
+              outp entered_GasAnalysis (snd (snd s), SID_GasAnalysis_Reading);
+              (do {skip ; stop} \<triangle>
+                (
+                \<comment> \<open> T_GasAnalysis_t0 \<close>
+                do {gs \<leftarrow> inp_in gas__GasAnalysis (set [(TID_GasAnalysis_t0, din, x). 
+                        x \<leftarrow> (lseq_gassensor_enum)]) ;
+                    outp set_gs_GasAnalysis (snd (snd gs));
+                    outp exit_GasAnalysis (SID_GasAnalysis_Reading, SID_GasAnalysis_Reading);
+                    outp exited_GasAnalysis (SID_GasAnalysis_Reading, SID_GasAnalysis_Reading);
+                    outp enter_GasAnalysis (SID_GasAnalysis_Reading, SID_GasAnalysis_Analysis);
+                    outp entered_GasAnalysis (SID_GasAnalysis_Reading, SID_GasAnalysis_Analysis);
+                    Ret(False, fst (snd s), SID_GasAnalysis_Reading)
+                    } \<box>
+                (exit_events_GasAnalysis (fst (snd s)) SID_GasAnalysis_Reading 
+                   tids_GasAnalysis_Reading Other_SIDs_to_Reading_GasAnalysis)
+                )
+              )
+            })
+            \<comment> \<open> The previous state: a triple \<close> 
+            (ret)
+        ) ;
+        Ret (id)
+  }
+)
+"
+
+definition State_GasAnalysis_Reading_R where
+"State_GasAnalysis_Reading_R (idd::integer) = 
+   (discard_state (State_GasAnalysis_Reading idd)) \<comment> \<open> discard state to match with skip on the right\<close>
+    \<parallel>\<^bsub> (int_int_GasAnalysis - GasAnalysis_Reading_triggers) \<^esub> 
+   skip
+"
+
+subsubsection \<open> State machine \<close>
+definition flow_events_GasAnalysis_stm_to_nodes where
+"flow_events_GasAnalysis_stm_to_nodes = (
+ let nodes = [SID_GasAnalysis_NoGas,SID_GasAnalysis_Analysis,SID_GasAnalysis_GasDetected,
+              SID_GasAnalysis_j1,SID_GasAnalysis_Reading]
+ in set (
+      enumchans2 [enter_GasAnalysis_C, entered_GasAnalysis_C,exit_GasAnalysis_C,exited_GasAnalysis_C] 
+          (filter (\<lambda> s. s \<notin> set nodes) SIDS_GasAnalysis_list) nodes
+  )
+)"
+
+definition STM_GasAnalysis where
+"STM_GasAnalysis (idd::integer) = 
+   (I_GasAnalysis_i1(idd))
+    \<parallel>\<^bsub> flow_events_GasAnalysis_stm_to_nodes \<^esub> 
+   (State_GasAnalysis_NoGas_R(idd)
+      \<parallel>\<^bsub> CS_GasAnalysis_Analysis_sync \<inter> (CS_GasAnalysis_Analysis_sync \<union> 
+          (CS_GasAnalysis_GasDetected_sync \<union> (CS_GasAnalysis_j1_sync \<union> CS_GasAnalysis_Reading_sync))) \<^esub>
+      (State_GasAnalysis_Analysis_R(idd)
+        \<parallel>\<^bsub> CS_GasAnalysis_Analysis_sync \<inter> (CS_GasAnalysis_GasDetected_sync \<union> 
+            (CS_GasAnalysis_j1_sync \<union> CS_GasAnalysis_Reading_sync)) \<^esub> 
+        ( State_GasAnalysis_GasDetected_R(idd)
+          \<parallel>\<^bsub> CS_GasAnalysis_GasDetected_sync \<inter> (CS_GasAnalysis_j1_sync \<union> CS_GasAnalysis_Reading_sync) \<^esub> 
+          (State_GasAnalysis_j1_R(idd)  
+            \<parallel>\<^bsub> CS_GasAnalysis_j1_sync \<inter> CS_GasAnalysis_Reading_sync \<^esub> 
+          State_GasAnalysis_Reading_R(idd))
+        )
+      )
+   )
+"
+
+definition GasAnalysis_opt_0_internal_set where
+"GasAnalysis_opt_0_internal_set = 
+  set (([internal_GasAnalysis_C TID_GasAnalysis_t1]) @ 
+       (enumchans3 [gas__GasAnalysis_C] 
+          [TID_GasAnalysis_t0, TID_GasAnalysis_t2] 
+          [din, dout] 
+          (lseq_gassensor_enum))
+)"
+
+definition GasAnalysis_opt_1_internal_set where
+"GasAnalysis_opt_1_internal_set = 
+  set ((enumchans1 [internal_GasAnalysis_C] [TID_GasAnalysis_t4, TID_GasAnalysis_t3]) @
+       (enumchans1 [set_st_GasAnalysis_C] Chemical_Status_list)
+)"
+
+definition GasAnalysis_opt_2_internal_set where
+"GasAnalysis_opt_2_internal_set = 
+  set ((enumchans1 [internal_GasAnalysis_C] [TID_GasAnalysis_t8, TID_GasAnalysis_t9a])
+)"
+
+definition MemorySTM_opt_GasAnalysis where
+"MemorySTM_opt_GasAnalysis (idd::integer) = 
+  (par_hide
+    (discard_state (GasAnalysis_Memory_opt_i (Chemical_IntensityC (0::2))))
+    GasAnalysis_i_events
+    (par_hide 
+      (par_hide
+        (discard_state (GasAnalysis_Memory_opt_st (Chemical_Status_noGas)))
+        GasAnalysis_st_events
+        (hide 
+          (
+            (hide
+              (
+                (par_hide
+                  (discard_state (GasAnalysis_Memory_opt_gs (bmake TYPE(2) [])))
+                  GasAnalysis_gs_events
+                  (par_hide 
+                    (discard_state (GasAnalysis_Memory_opt_a Chemical_Angle_Left)) 
+                    GasAnalysis_a_events 
+                    (STM_GasAnalysis idd)
+                  )
+                )
+                \<parallel>\<^bsub> GasAnalysis_opt_0_internal_set \<^esub>
+                (discard_state (GasAnalysis_MemoryTransitions_opt_0 idd))
+              )
+              ({internal_GasAnalysis_C TID_GasAnalysis_t1})
+            )
+            \<parallel>\<^bsub> GasAnalysis_opt_1_internal_set \<^esub> 
+            (discard_state (GasAnalysis_MemoryTransitions_opt_1 idd))
+          )
+          (set (enumchans1 [internal_GasAnalysis_C] [TID_GasAnalysis_t4, TID_GasAnalysis_t3]))
+        )
+      )
+      GasAnalysis_opt_2_internal_set
+      (discard_state (GasAnalysis_MemoryTransitions_opt_2 idd))
+    )
+  )   
+"
+
+definition rename_GasAnalysis_events where
+"rename_GasAnalysis_events = 
+  concat (
+    (enumchan2 (forget_first2 gas__GasAnalysis_C gas_GasAnalysis_C TIDS_GasAnalysis_list) 
+            InOut_list lseq_gassensor_enum) @
+    (enumchan2 (forget_first2 turn__GasAnalysis_C turn_GasAnalysis_C TIDS_GasAnalysis_list) 
+            InOut_list Chemical_Angle_list) @
+    (enumchan1 (forget_first resume__GasAnalysis_C resume_GasAnalysis_C TIDS_GasAnalysis_list) 
+            InOut_list) @
+    (enumchan1 (forget_first stop__GasAnalysis_C stop_GasAnalysis_C TIDS_GasAnalysis_list) 
+            InOut_list)
+  )
+"
+
+term "\<lbrace>resume__GasAnalysis (t, x) \<mapsto> resume_GasAnalysis x | (x, t). x \<in> InOut_set\<rbrace>"
+term "\<lbrace>terminate_GasAnalysis () \<mapsto> terminate_GasAnalysis () | _. True\<rbrace>"
+
+definition rename_GasAnalysis_events_others where
+"rename_GasAnalysis_events_others = 
+  (enumchanp1 terminate_GasAnalysis_C [()]) @
+  (enumchansp1 [get_i_GasAnalysis_C, set_i_GasAnalysis_C] Chemical_Intensity2_list) @
+  (enumchansp1 [get_a_GasAnalysis_C, set_a_GasAnalysis_C] Chemical_Angle_list) @
+  (enumchansp1 [get_st_GasAnalysis_C, set_st_GasAnalysis_C] Chemical_Status_list) @
+  (enumchansp1 [get_gs_GasAnalysis_C, set_gs_GasAnalysis_C] lseq_gassensor_enum) @
+  (enumchansp2 [gas_GasAnalysis_C] InOut_list lseq_gassensor_enum) @
+  (enumchansp2 [turn_GasAnalysis_C] InOut_list Chemical_Angle_list) @
+  (enumchansp1 [resume_GasAnalysis_C, stop_GasAnalysis_C] InOut_list) @
+  (enumchansp2 [enter_GasAnalysis_C, entered_GasAnalysis_C, exit_GasAnalysis_C, exited_GasAnalysis_C] 
+    SIDS_GasAnalysis_list SIDS_GasAnalysis_list) @
+  (enumchansp1 [internal_GasAnalysis_C] TIDS_GasAnalysis_list)
+"
+
+definition rename_MemorySTM_opt_GasAnalysis where
+"rename_MemorySTM_opt_GasAnalysis idd = 
+  rename (set (rename_GasAnalysis_events @ rename_GasAnalysis_events_others)) 
+    (MemorySTM_opt_GasAnalysis idd)
+"
+
+definition AUX_opt_GasAnalysis where
+"AUX_opt_GasAnalysis (idd::integer) = 
+  (hide 
+    ( 
+      (rename_MemorySTM_opt_GasAnalysis idd) \<lbrakk> set [terminate_GasAnalysis_C ()] \<Zrres> skip
+    )
+    GasAnalysis_MachineInternalEvents
+  )
+"
+
+definition D__GasAnalysis where
+"D__GasAnalysis (idd::integer) = 
+  hide (AUX_opt_GasAnalysis idd) internal_events_GasAnalysis
+"
+
+subsection \<open> MainController \<close>
+chantype Chan_MainCtrl =
+  terminate_MainCtrl :: unit
+  gas_MainCtrl :: "InOut \<times> 2 Chemical_GasSensor[2]blist"
+  resume_MainCtrl :: "InOut"
+  turn_MainCtrl :: "InOut \<times> Chemical_Angle"
+  stop_MainCtrl :: "InOut"
+
+subsubsection \<open> Memory \<close>
+definition Memory_MainCtrl where
+"Memory_MainCtrl (idd::integer) = skip"
+
+subsubsection \<open> Controller \<close>
+
+definition rename_MainCtrl_GasAnalysis_events where
+"rename_MainCtrl_GasAnalysis_events = 
+  (enumchanp2_1 (terminate_GasAnalysis_C,terminate_MainCtrl_C) [()]) @
+  (enumchansp2_2 [(gas_GasAnalysis_C, gas_MainCtrl_C)] InOut_list lseq_gassensor_enum) @
+  (enumchansp2_1 [(resume_GasAnalysis_C, resume_MainCtrl_C)] InOut_list) @
+  (enumchansp2_2 [(turn_GasAnalysis_C, turn_MainCtrl_C)] InOut_list Chemical_Angle_list) @
+  (enumchansp2_1 [(stop_GasAnalysis_C, stop_MainCtrl_C)] InOut_list)
+"
+
+definition rename_D__GasAnalysis where
+  "rename_D__GasAnalysis idd = rename (set rename_MainCtrl_GasAnalysis_events) (D__GasAnalysis idd)"
+
+definition D__MainCtrl where
+"D__MainCtrl (idd::integer) = 
+  (par_hide
+    (rename_D__GasAnalysis idd)
+    {}
+    (discard_state (Memory_MainCtrl idd))
+  )  \<lbrakk> set [terminate_MainCtrl_C ()] \<Zrres> skip
+"
+
+export_code
+  GasAnalysis_Memory_opt_gs
+  GasAnalysis_MemoryTransitions_opt_0
+  GasAnalysis_MemoryTransitions_opt_1
+  GasAnalysis_MemoryTransitions_opt_2
+  I_GasAnalysis_i1
+  State_GasAnalysis_NoGas
+  State_GasAnalysis_NoGas_R
+  State_GasAnalysis_Analysis_R
+  State_GasAnalysis_GasDetected_R
+  State_GasAnalysis_j1_R
+  State_GasAnalysis_Reading_R
+  MemorySTM_opt_GasAnalysis
+  AUX_opt_GasAnalysis
+  D__GasAnalysis
+in Haskell 
+  (* module_name GasAnalysis *)
+  file_prefix RoboChart_ChemicalDetector 
+  (string_classes) 
+
+end
